typechecker progress

theories/typechecker/typechecker.v
@@ -339,7 +339,7 @@ Ltac find_Forall_foldr checker prop :=
       solve_Forall_foldr HForall Hfoldr checker prop
   end.
 
-Lemma type_ok_checker_correct :
+Lemma type_ok_checker_correct_basic :
   (forall t F, (type_ok_checker F t = ok_term) -> type_ok F t) /\
   (forall ft F, function_type_ok_checker F ft = ok_term -> function_type_ok F ft).
 Proof.
@@ -360,12 +360,2419 @@ Proof.
 
 Qed.
 
+Lemma type_ok_checker_correct :
+  ∀ t F, (type_ok_checker F t = ok_term) -> type_ok F t.
+Proof.
+  apply type_ok_checker_correct_basic.
+Qed.
 
-(* Have to define an equality operator on representation and dropability *)
-Fixpoint subkind_of_checker (κ1:kind) (κ2:kind) : type_checker_res :=
+Lemma function_type_ok_checker_correct :
+  ∀ ft F, function_type_ok_checker F ft = ok_term -> function_type_ok F ft.
+Proof.
+  apply type_ok_checker_correct_basic.
+Qed.
+
+Scheme Equality for copyability.
+Scheme Equality for dropability.
+Scheme Equality for atomic_rep.
+Scheme Equality for base_memory.
+Scheme Equality for memory.
+
+Scheme Equality for list.
+
+
+Fixpoint representation_beq (r1:representation) (r2:representation) : bool :=
+  match r1, r2 with
+  | VarR i1, VarR i2 => (i1 =? i2)
+  | SumR r1s, SumR r2s => list_beq representation representation_beq r1s r2s
+  | ProdR r1s, ProdR r2s => list_beq representation representation_beq r1s r2s
+  | AtomR a1, AtomR a2 => atomic_rep_beq a1 a2
+  | _, _ => false
+  end.
+
+Lemma representation_eq_convert :
+  ∀ r1 r2, representation_beq r1 r2 = true <-> r1 = r2.
+Proof.
+  split; intros.
+  - induction r1 using rep_ind; induction r2 using rep_ind; simpl in H; try inversion H.
+    * apply Nat.eqb_eq in H; by subst.
+    * (* okay this is doable, but not worth it rn *)
+      admit.
+    * admit.
+    * (* doable almost certainly *) admit.
+  - subst.
+    induction r2 using rep_ind.
+    * simpl. by apply Nat.eqb_eq.
+    * simpl. (* it gotta be but not worth it rn honestly *)
+Admitted.
+
+Fixpoint size_beq (s1:size) (s2:size) : bool :=
+  match s1, s2 with
+  | VarS i1, VarS i2 => (i1 =? i2)
+  | SumS s1s, SumS s2s => list_beq size size_beq s1s s2s
+  | ProdS s1s, ProdS s2s => list_beq size size_beq s1s s2s
+  | RepS r1, RepS r2 => representation_beq r1 r2
+  | ConstS n1, ConstS n2 => (n1 =? n2)
+  | _, _ => false
+  end.
+
+Lemma size_eq_convert :
+  ∀ s1 s2, size_beq s1 s2 = true <-> s1 = s2.
+Proof.
+Admitted.
+
+Fixpoint kind_beq (k1:kind) (k2:kind) : bool :=
+  match k1, k2 with
+  | VALTYPE r1 c1 d1, VALTYPE r2 c2 d2 =>
+      andb (representation_beq r1 r2) (andb (copyability_beq c1 c2) (dropability_beq d1 d2))
+  | MEMTYPE s1 d1, MEMTYPE s2 d2 =>
+      andb (size_beq s1 s2) (dropability_beq d1 d2)
+  | _, _ => false
+  end.
+
+Lemma kind_eq_convert :
+  ∀ k1 k2, kind_beq k1 k2 = true <-> k1 = k2.
+Proof. Admitted.
+
+Lemma kind_neq_convert :
+  ∀ k1 k2, kind_beq k1 k2 = false <-> k1 <> k2.
+Proof.
+  split; intros.
+  (* there's some decidability lemmas that need to be done. This is fine to leave. *)
+Admitted.
+
+
+Definition mono_mem_checker (μ:memory) : type_checker_res :=
+  match μ with
+  | BaseM bm => ok_term
+  | _ => INR "not monomem"
+  end.
+
+(* This is using the above custom representation and size *)
+Definition subkind_of_checker (κ1:kind) (κ2:kind) : type_checker_res :=
   match κ1, κ2 with
   | (VALTYPE ρ1 ImCopy δ1), (VALTYPE ρ2 ExCopy δ2) =>
-      (* this true here is fake *)
-      if true then ok_term else INR "not subkind"
+      if andb (representation_beq ρ1 ρ2) (dropability_beq δ1 δ2)
+      then ok_term else INR "fail in subkind check"
+  | (VALTYPE ρ1 ExCopy δ1), (VALTYPE ρ2 NoCopy δ2) =>
+      if andb (representation_beq ρ1 ρ2) (dropability_beq δ1 δ2)
+      then ok_term else INR "fail in subkind check"
+  | (VALTYPE ρ1 χ1 ImDrop), (VALTYPE ρ2 χ2 ExDrop) =>
+      if andb (representation_beq ρ1 ρ2) (copyability_beq χ1 χ2)
+      then ok_term else INR "fail in subkind check"
+  | (MEMTYPE σ1 ImDrop), (MEMTYPE σ2 ExDrop) =>
+      if size_beq σ1 σ2
+      then ok_term else INR "fail in subkind check"
   | _, _ => INR "no"
   end.
+
+
+Lemma dropability_eq_convert :
+  ∀ d1 d2, dropability_beq d1 d2 = true <-> d1 = d2.
+Proof.
+  split; intros.
+  - by apply internal_dropability_dec_bl in H.
+  - by apply internal_dropability_dec_lb in H.
+Qed.
+
+Lemma copyability_eq_convert :
+  ∀ c1 c2, copyability_beq c1 c2 = true <-> c1 = c2.
+Proof.
+  split; intros;
+    [by apply internal_copyability_dec_bl in H | by apply internal_copyability_dec_lb in H].
+Qed.
+
+Lemma memory_eq_convert :
+  ∀ m1 m2, memory_beq m1 m2 = true <-> m1 = m2.
+Proof. Admitted.
+
+
+Ltac my_auto2 :=
+  match goal with
+  | H: ((match ?key with |_=>_ end) = _) |- _ => destruct key eqn:?HMatch; [ | inversion H ]; simpl in *
+  | H: ((match ?key with |_=>_ end) = _) |- _ => destruct key eqn:?HMatch; [ inversion H | ]; simpl in *
+  | H:((if ?key then _ else _)=_) |- _ => destruct key eqn:?HMatch; [ | inversion H ]
+  | o:ok |- _ => stupid_unit o
+  | H: ok_term = ok_term |- _ => clear H
+  | H: (andb _ _ = true) |- _ => apply andb_prop in H; destruct H as [?H1 ?H2]
+  | H: (_ && _ = true) |- _ => apply andb_prop in H; destruct H as [?H1 ?H2]
+  | H: true = false |- _ => inversion H
+  | H: false = true |- _ => inversion H
+  | H: (representation_beq _ _ = true) |- _ => apply representation_eq_convert in H; subst; auto
+  | H: (dropability_beq _ _ = true) |- _ => apply dropability_eq_convert in H; subst; auto
+  | H: (copyability_beq _ _ = true) |- _ => apply copyability_eq_convert in H; subst; auto
+  | H: (size_beq _ _ = true) |- _ => apply size_eq_convert in H; subst; auto
+  | H: (kind_ok_checker _ _ = inl ()) |- _ => apply kind_ok_checker_correct in H; auto
+  | H: (kind_ok_checker _ _ = ok_term) |- _ => apply kind_ok_checker_correct in H; auto
+  | H: (mem_ok_checker _ _ = inl ()) |- _ => apply mem_ok_checker_correct in H; auto
+  | H: (mem_ok_checker _ _ = ok_term) |- _ => apply mem_ok_checker_correct in H; auto
+  | H: (rep_ok_checker _ _ = inl ()) |- _ => apply rep_ok_checker_correct in H; auto
+  | H: (rep_ok_checker _ _ = ok_term) |- _ => apply rep_ok_checker_correct in H; auto
+  | H: (size_ok_checker _ _ = inl ()) |- _ => apply size_ok_checker_correct in H; auto
+  | H: (size_ok_checker _ _ = ok_term) |- _ => apply size_ok_checker_correct in H; auto
+  | H: (type_ok_checker _ _ = inl ()) |- _ => apply type_ok_checker_correct in H; auto
+  | H: (type_ok_checker _ _ = ok_term) |- _ => apply type_ok_checker_correct in H; auto
+  | H: (function_type_ok_checker _ _ = inl ()) |- _ => apply function_type_ok_checker_correct in H; auto
+  | H: (function_type_ok_checker _ _ = ok_term) |- _ => apply function_type_ok_checker_correct in H; auto
+end.
+
+
+Lemma subkind_of_checker_correct :
+  ∀ k1 k2, subkind_of_checker k1 k2 = ok_term -> subkind_of k1 k2.
+Proof.
+  intros.
+  destruct k1, k2;
+    try destruct c, c0; try destruct d, d0; simpl in H; try inversion H;
+    repeat my_auto2;
+    try apply KSubValExCopy; try apply KSubValNoCopy; try apply KSubValExDrop; try apply KSubMemExDrop;
+    repeat my_auto2.
+  1-4: destruct c; simpl in *; inversion H.
+Qed.
+
+Definition has_kind_ok_checker (F:function_ctx) (t:type) (k:kind) : type_checker_res :=
+  match (type_ok_checker F t) with
+  | inl () => (kind_ok_checker (F.(fc_kind_ctx)) k)
+  | err => err
+  end.
+
+Lemma has_kind_ok_checker_correct :
+  ∀ F t k, has_kind_ok_checker F t k = ok_term -> has_kind_ok F t k.
+Proof.
+  intros. unfold has_kind_ok_checker in H. repeat my_auto2.
+  constructor; auto.
+Qed.
+
+
+
+(* Time for has-kind oh boy oh boy *)
+
+
+(* This function just grabs the kind out of the type *)
+Definition grab_kind (F:function_ctx) (t:type) : option kind :=
+  match t with
+  | I31T k => Some k
+  | NumT k _ => Some k
+  | SumT k _ => Some k
+  | VariantT k _ => Some k
+  | ProdT k _ => Some k
+  | StructT k _ => Some k
+  | RefT k _ _ => Some k
+  | CodeRefT k _ => Some k
+  | SerT k _ => Some k
+  | PlugT k _ => Some k
+  | SpanT k _ => Some k
+  | RecT k _ => Some k
+  | ExistsMemT k _ => Some k
+  | ExistsRepT k _ => Some k
+  | ExistsSizeT k _ => Some k
+  | ExistsTypeT k _ _ => Some k
+  | VarT t => (F.(fc_type_vars)) !! t
+  end.
+
+
+(* A thing that helps with subkinding *)
+Definition check_if_subkind (k1:kind) (k2:kind) : type_checker_res :=
+  match k1, k2 with
+  | VALTYPE ρ1 χ1 δ1, VALTYPE ρ2 χ2 δ2 =>
+      if representation_beq ρ1 ρ2
+      then
+        match χ1, χ2 with
+        | ImCopy, _
+        | ExCopy, ExCopy
+        | ExCopy, NoCopy
+        | NoCopy, NoCopy =>
+            match δ1, δ2 with
+            | ImDrop, _
+            | ExDrop, ExDrop => ok_term
+            | _, _ => INR "not subkind"
+            end
+        | _, _ => INR "not subkind"
+        end
+      else INR "mismatch in representation for subkinds"
+  | MEMTYPE σ1 δ1, MEMTYPE σ2 δ2 =>
+      if size_beq σ1 σ2
+      then
+        match δ1, δ2 with
+        | ImDrop, _
+        | ExDrop, ExDrop => ok_term
+        | _, _ => INR "not subkind"
+        end
+      else INR "mismatch in sizity for subkinds"
+  | _, _ => INR "mismatch in general kind for subkind"
+  end.
+
+Lemma check_if_subkind_works_with_has_kind :
+  ∀ F τ k1 k2,
+    check_if_subkind k1 k2 = ok_term ->
+    has_kind F τ k1 ->
+    has_kind F τ k2.
+Proof.
+  intros.
+  destruct k1, k2; simpl in H; inversion H.
+  - repeat my_auto2. rename r0 into r.
+    destruct c, c0, d, d0; simpl in *; auto; repeat my_auto2; try inversion H.
+    (* Look I know this probably should be ltacable but I couldn't be bothered *)
+    + apply (KSub _ _ (VALTYPE r NoCopy ImDrop) _); try constructor; auto.
+    + apply (KSub _ _ (VALTYPE r ExCopy ExDrop) _); try constructor; auto.
+    + apply (KSub _ _ (VALTYPE r ExCopy ExDrop) _); try constructor; auto.
+      apply (KSub _ _ (VALTYPE r ExCopy ImDrop) _); try constructor; auto.
+    + apply (KSub _ _ (VALTYPE r ExCopy ImDrop) _); try constructor; auto.
+    + apply (KSub _ _ (VALTYPE r ExCopy ImDrop) _); try constructor; auto.
+    + apply (KSub _ _ (VALTYPE r ExCopy ExDrop) _); try constructor; auto.
+      apply (KSub _ _ (VALTYPE r ImCopy ExDrop) _); try constructor; auto.
+    + apply (KSub _ _ (VALTYPE r ExCopy ExDrop) _); try constructor; auto.
+      apply (KSub _ _ (VALTYPE r ExCopy ImDrop) _); try constructor; auto.
+      apply (KSub _ _ (VALTYPE r ImCopy ImDrop) _); try constructor; auto.
+    + apply (KSub _ _ (VALTYPE r ExCopy ImDrop) _); try constructor; auto.
+      apply (KSub _ _ (VALTYPE r ImCopy ImDrop) _); try constructor; auto.
+    + apply (KSub _ _ (VALTYPE r ImCopy ExDrop) _); try constructor; auto.
+    + apply (KSub _ _ (VALTYPE r ExCopy ImDrop) _); try constructor; auto.
+      apply (KSub _ _ (VALTYPE r ImCopy ImDrop) _); try constructor; auto.
+    + apply (KSub _ _ (VALTYPE r ImCopy ImDrop) _); try constructor; auto.
+    + apply (KSub _ _ (VALTYPE r ImCopy ImDrop) _); try constructor; auto.
+  - repeat my_auto2.
+    destruct d0; auto.
+    apply (KSub _ _ (MEMTYPE s0 ImDrop) _); try constructor; auto.
+Qed.
+
+
+
+Fixpoint foldr2 {A B C : Type} (f : B → C → A → A) (a0 : A)
+  (lB : list B) (lC : list C) :=
+  match lB, lC with
+  | b :: lB0, c :: lC0 => f b c (foldr2 f a0 lB0 lC0)
+  | _, _ => a0
+  end.
+
+
+(* Check kind in a naive way. I guess. *)
+Fixpoint has_kind_checker (F:function_ctx) (t:type) (k:kind) : type_checker_res :=
+  match t with
+  | VarT t =>
+      match (F.(fc_type_vars)) !! t with
+      | Some κ =>
+          match kind_ok_checker (F.(fc_kind_ctx)) κ with
+          | inl () => check_if_subkind κ k
+          | err => err
+          end
+      | None => INR "variable not in there or smthn"
+      end
+  (* Numbers *)
+  | I31T κ =>
+      if (kind_beq κ (VALTYPE (AtomR PtrR) ImCopy ImDrop))
+      then check_if_subkind κ k
+      else INR "wrong kind for I31T"
+    (* NumT *)
+  | NumT κ (IntT I32T) =>
+      if (kind_beq κ (VALTYPE (AtomR I32R) ImCopy ImDrop))
+      then check_if_subkind κ k
+      else INR "wrong kind for I32T"
+  | NumT κ (IntT I64T) =>
+      if (kind_beq κ (VALTYPE (AtomR I64R) ImCopy ImDrop) )
+      then check_if_subkind κ k
+      else INR "wrong kind for I64T"
+  | NumT κ (FloatT F32T) =>
+      if (kind_beq κ (VALTYPE (AtomR F32R) ImCopy ImDrop))
+      then check_if_subkind κ k
+      else INR "wrong kind for F32T"
+  | NumT κ (FloatT F64T) =>
+      if (kind_beq κ (VALTYPE (AtomR F64R) ImCopy ImDrop))
+      then check_if_subkind κ k
+      else INR "wrong kind for F64T"
+  (* Sums and Prods *)
+  | SumT κ τs =>
+      match κ with
+      | VALTYPE (SumR ρs) χ δ =>
+          if foldr2
+               (λ t:type, λ r:representation,
+                  andb (check_ok_output (has_kind_checker F t (VALTYPE r χ δ)))
+               ) true τs ρs
+          then check_if_subkind κ k
+          else INR "bad sum kind internals"
+      | _ => INR "bad sum kind format"
+      end
+  | VariantT κ τs =>
+      match κ with
+      | MEMTYPE (SumS σs) δ =>
+          if foldr2
+               (λ t:type, λ s:size,
+                  andb (check_ok_output (has_kind_checker F t (MEMTYPE s δ)))
+               ) true τs σs
+          then check_if_subkind κ k
+          else INR "bad sum kind internals"
+      | _ => INR "bad variant kind format"
+      end
+   | ProdT κ τs =>
+      match κ with
+      | VALTYPE (ProdR ρs) χ δ =>
+          if foldr2
+               (λ t:type, λ r:representation,
+                  andb (check_ok_output (has_kind_checker F t (VALTYPE r χ δ)))
+               ) true τs ρs
+          then check_if_subkind κ k
+          else INR "bad sum kind internals"
+      | _ => INR "bad prod kind format"
+      end
+  | StructT κ τs =>
+      match κ with
+      | MEMTYPE (ProdS σs) δ =>
+          if foldr2
+               (λ t:type, λ s:size,
+                  andb (check_ok_output (has_kind_checker F t (MEMTYPE s δ)))
+               ) true τs σs
+          then check_if_subkind κ k
+          else INR "bad sum kind internals"
+      | _ => INR "bad struct kind format"
+      end
+  (* References *)
+  | RefT κ (BaseM MemGC) τ =>
+      if (kind_beq κ (VALTYPE (AtomR PtrR) ExCopy ExDrop))
+      then
+        match grab_kind F τ with
+          | Some innerk =>
+              match innerk with
+              | MEMTYPE σ δ =>
+                  match has_kind_checker F τ (MEMTYPE σ δ) with
+                  | inl () => check_if_subkind κ k
+                  | err => err
+                  end
+              | _ => INR "you have a reft t where t isnt memtype"
+              end
+          | None => INR "i think you have a bad variable or smthn"
+          end
+      else INR "bad gc mem kind format"
+  | RefT κ μ τ =>
+      if (kind_beq κ (VALTYPE (AtomR PtrR) NoCopy ExDrop))
+      then
+        match mem_ok_checker (F.(fc_kind_ctx)) μ with
+          | inl () =>
+              match grab_kind F τ with
+              | Some innerk =>
+                  match innerk with
+                  | MEMTYPE σ δ =>
+                      match has_kind_checker F τ (MEMTYPE σ δ) with
+                      | inl () => check_if_subkind κ k
+                      | err => err
+                      end
+                  | _ => INR "you have ref t where t isnt memtype"
+                  end
+              | None => INR "i think you have a bad variable or smthn"
+              end
+          | err => err
+          end
+      else INR "bad ref kind format"
+  | CodeRefT κ ϕ =>
+      match κ with
+      | VALTYPE (AtomR I32R) ImCopy ImDrop =>
+          match function_type_ok_checker F ϕ with
+          | inl () => check_if_subkind κ k
+          | err => err
+          end
+      | _ => INR "bad coderef kind format"
+      end
+  (* Some weird ones I guess *)
+  | SerT κ τ =>
+      match κ with
+      | MEMTYPE (RepS ρ) δ =>
+          match has_kind_checker F τ (VALTYPE ρ ImCopy δ) with
+          | inl () => check_if_subkind κ k
+          | err => err
+          end
+      | _ => INR "bad ser kind format"
+      end
+  | PlugT κ ρ =>
+      match κ with
+      | VALTYPE ρ1 ImCopy ImDrop =>
+          if representation_beq ρ ρ1
+          then
+            match rep_ok_checker (F.(fc_kind_ctx)) ρ with
+            | inl () => check_if_subkind κ k
+            | err => err
+            end
+          else INR "plug's rep doesn't match kind's rep"
+      | _ => INR "bad plug kind format"
+      end
+  | SpanT κ σ =>
+      match κ with
+      | MEMTYPE σ1 ImDrop =>
+          if size_beq σ σ1
+          then
+            match size_ok_checker (F.(fc_kind_ctx)) σ with
+            | inl () => check_if_subkind κ k
+            | err => err
+            end
+          else INR "span's size doesn't match kind's size"
+      | _ => INR "bad span kind format"
+      end
+  | RecT κ τ =>
+      match has_kind_checker (F <| fc_type_vars ::= cons κ |>) τ κ with
+      | inl () => check_if_subkind κ k
+      | err => err
+      end
+  | ExistsMemT κ τ =>
+      match kind_ok_checker (F.(fc_kind_ctx)) κ with
+      | inl () =>
+          match has_kind_checker (F <| fc_kind_ctx ::= set kc_mem_vars S |>) τ κ with
+          | inl () => check_if_subkind κ k
+          | err => err
+          end
+      | err => err
+      end
+  | ExistsRepT κ τ =>
+      match kind_ok_checker (F.(fc_kind_ctx)) κ with
+      | inl () =>
+          match has_kind_checker (F <| fc_kind_ctx ::= set kc_rep_vars S |>) τ κ with
+          | inl () => check_if_subkind κ k
+          | err => err
+          end
+      | err => err
+      end
+   | ExistsSizeT κ τ =>
+      match kind_ok_checker (F.(fc_kind_ctx)) κ with
+      | inl () =>
+          match has_kind_checker (F <| fc_kind_ctx ::= set kc_size_vars S |>) τ κ with
+          | inl () => check_if_subkind κ k
+          | err => err
+          end
+      | err => err
+      end
+  | ExistsTypeT κ κ0 τ =>
+      match kind_ok_checker (F.(fc_kind_ctx)) κ with
+      | inl () =>
+          match kind_ok_checker (F.(fc_kind_ctx)) κ0 with
+          | inl () =>
+              match has_kind_checker (F <| fc_type_vars ::= cons κ0 |>) τ κ with
+              | inl () => check_if_subkind κ k
+              | err => err
+              end
+          | err => err
+          end
+      | err => err
+      end
+  end.
+
+Ltac my_auto3 :=
+  match goal with
+  | H: ((match ?key with |_=>_ end) = _) |- _ => destruct key eqn:?HMatch; try inversion H; simpl in *
+  | H:((if ?key then _ else _)=_) |- _ => destruct key eqn:?HMatch; try inversion H; simpl in *
+  | H: (kind_beq _ _ = true) |- _ => apply kind_eq_convert in H; subst; auto
+  | o:ok |- _ => stupid_unit o
+  | H: ok_term = ok_term |- _ => clear H
+  | H: (andb _ _ = true) |- _ => apply andb_prop in H; destruct H as [?H1 ?H2]
+  | H: (_ && _ = true) |- _ => apply andb_prop in H; destruct H as [?H1 ?H2]
+  | H: true = false |- _ => inversion H
+  | H: false = true |- _ => inversion H
+  | H: (representation_beq _ _ = true) |- _ => apply representation_eq_convert in H; subst; auto
+  | H: (dropability_beq _ _ = true) |- _ => apply dropability_eq_convert in H; subst; auto
+  | H: (copyability_beq _ _ = true) |- _ => apply copyability_eq_convert in H; subst; auto
+  | H: (size_beq _ _ = true) |- _ => apply size_eq_convert in H; subst; auto
+  | H: (kind_ok_checker _ _ = inl ()) |- _ => apply kind_ok_checker_correct in H; auto
+  | H: (kind_ok_checker _ _ = ok_term) |- _ => apply kind_ok_checker_correct in H; auto
+  | H: (mem_ok_checker _ _ = inl ()) |- _ => apply mem_ok_checker_correct in H; auto
+  | H: (mem_ok_checker _ _ = ok_term) |- _ => apply mem_ok_checker_correct in H; auto
+  | H: (rep_ok_checker _ _ = inl ()) |- _ => apply rep_ok_checker_correct in H; auto
+  | H: (rep_ok_checker _ _ = ok_term) |- _ => apply rep_ok_checker_correct in H; auto
+  | H: (size_ok_checker _ _ = inl ()) |- _ => apply size_ok_checker_correct in H; auto
+  | H: (size_ok_checker _ _ = ok_term) |- _ => apply size_ok_checker_correct in H; auto
+  | H: (type_ok_checker _ _ = inl ()) |- _ => apply type_ok_checker_correct in H; auto
+  | H: (type_ok_checker _ _ = ok_term) |- _ => apply type_ok_checker_correct in H; auto
+  | H: (function_type_ok_checker _ _ = inl ()) |- _ => apply function_type_ok_checker_correct in H; auto
+  | H: (function_type_ok_checker _ _ = ok_term) |- _ => apply function_type_ok_checker_correct in H; auto
+  | H: (check_if_subkind _ _ = inl ()) |- _ =>
+      try( by (eapply check_if_subkind_works_with_has_kind; try constructor; auto))
+  | H: (check_if_subkind _ _ = ok_term) |- _ =>
+      try( by (eapply check_if_subkind_works_with_has_kind; try constructor; auto))
+  | H: (INR _ = ok_term) |- _ => inversion H
+  | H: (INR _ = inl ()) |- _ => inversion H
+end.
+
+Opaque check_if_subkind.
+Opaque mem_ok_checker.
+(* this needs to not be unravelled by any tactics. Makes
+ automation a lot easier *)
+
+
+(* The stupid True is there bc idk how to make the induction work otherwise *)
+Lemma has_kind_checker_correct_basic :
+  (∀ t F k, has_kind_checker F t k = ok_term -> has_kind F t k) /\
+  (∀ (ft:function_type) (F:function_ctx), True  ).
+Proof.
+  apply type_and_function_ind; intros; simpl in *; auto; repeat my_auto3.
+  (* The following 4 (sums and prods) will rely on some foldr2 lemma *)
+  (* I will do that later *)
+  1-4: admit.
+
+  (* then these actually need the simple inductive hyp *)
+  1-4: match goal with
+    | HSTAR: (has_kind_checker _ _ _ = _) |- _ => apply H in HSTAR
+    end.
+  1-2: eapply check_if_subkind_works_with_has_kind; [apply H0 | apply (KRef _ _ _ s d); auto].
+  1: eapply check_if_subkind_works_with_has_kind; [apply H0 | apply (KRefGC _ _ s d); auto].
+
+  (* Just ser *)
+  eapply check_if_subkind_works_with_has_kind; [apply H0 | eapply KSer; apply HMatch1 ].
+
+Admitted.
+
+Lemma has_kind_checker_correct :
+  ∀ F t k, has_kind_checker F t k = ok_term -> has_kind F t k.
+Proof.
+  pose proof has_kind_checker_correct_basic.
+  destruct H; auto.
+Qed.
+
+
+(* Small things before pathing *)
+Definition has_rep_checker F τ ρ : type_checker_res :=
+  has_kind_checker F τ (VALTYPE ρ ImCopy ImDrop).
+
+Lemma has_rep_checker_correct :
+  ∀ F τ ρ, has_rep_checker F τ ρ = ok_term -> has_rep F τ ρ.
+Proof.
+  intros.
+  unfold has_rep_checker in H.
+  apply has_kind_checker_correct in H.
+  apply (RepVALTYPE _ _ _ ImCopy ImDrop); auto.
+Qed.
+
+Definition grab_rep F τ : option representation :=
+  match grab_kind F τ with
+  | Some κ =>
+      match κ with
+      | VALTYPE ρ _ _ => Some ρ
+      | _ => None
+      end
+  | None => None
+  end.
+
+Definition is_mono_rep_checker :=
+  rep_ok_checker kc_empty.
+
+Definition has_mono_rep_checker F τ : type_checker_res :=
+  match grab_rep F τ with
+  | Some ρ =>
+      match has_rep_checker F τ ρ with
+      | inl () => is_mono_rep_checker ρ
+      | err => err
+      end
+  | None => INR "youre checking mono rep for something that is not valtype or smthn similar"
+  end.
+
+Lemma has_mono_rep_checker_correct :
+  ∀ F τ, has_mono_rep_checker F τ = ok_term -> has_mono_rep F τ.
+Proof.
+  intros. unfold has_mono_rep_checker in H.
+  repeat my_auto3.
+  unfold is_mono_rep_checker in *.
+  repeat my_auto3.
+  apply has_rep_checker_correct in HMatch0.
+  apply (MonoRep _ _ r); auto.
+Qed.
+
+Definition has_mono_rep_instr_checker F inst : type_checker_res :=
+  match inst with
+  | InstrT τs1 τs2 =>
+      if (foldr (λ t:type, andb (check_ok (has_mono_rep_checker F) t)) true τs1)
+      then
+        if (foldr (λ t:type, andb (check_ok (has_mono_rep_checker F) t)) true τs2)
+        then ok_term
+        else INR "function type ok error"
+      else INR "function type ok error"
+  end.
+
+Lemma has_mono_rep_instr_checker_correct :
+  ∀ F inst, has_mono_rep_instr_checker F inst = ok_term -> has_mono_rep_instr F inst.
+Proof.
+  intros.
+  unfold has_mono_rep_instr_checker in *.
+  repeat my_auto3. pose proof has_mono_rep_checker_correct.
+  split; [clear HMatch1 | clear HMatch0].
+  - (* yeah this is true but I dont wanna prove it *)
+    admit.
+  - admit.
+Admitted.
+
+Definition grab_size F τ : option size :=
+  match grab_kind F τ with
+  | Some κ =>
+      match κ with
+      | MEMTYPE σ _ => Some σ
+      | _ => None
+      end
+  | None => None
+  end.
+
+Definition has_size_checker F τ σ : type_checker_res :=
+  has_kind_checker F τ (MEMTYPE σ ImDrop).
+
+Lemma has_size_checker_correct :
+  ∀ F τ σ, has_size_checker F τ σ = ok_term -> has_size F τ σ.
+Proof.
+  intros. unfold has_size_checker in H.
+  apply has_kind_checker_correct in H.
+  unfold has_size.
+  by exists ImDrop.
+Qed.
+
+Definition is_mono_size_checker := size_ok_checker kc_empty.
+
+Definition has_mono_size_checker F τ : type_checker_res :=
+  match grab_size F τ with
+  | Some σ =>
+      match has_size_checker F τ σ with
+      | inl () => is_mono_size_checker σ
+      | err => err
+      end
+  | None => INR "youre checking mono size for something that is not memtype or smthn similar"
+  end.
+
+Lemma has_mono_size_checker_correct :
+  ∀ F τ, has_mono_size_checker F τ = ok_term -> has_mono_size F τ.
+Proof.
+  intros.
+  unfold has_mono_size_checker in *.
+  repeat my_auto3.
+  unfold is_mono_size_checker in *. unfold has_size_checker in *.
+  repeat my_auto3. apply has_kind_checker_correct in HMatch0.
+  by apply (MonoSizeMEMTYPE _ _ s ImDrop).
+Qed.
+
+Scheme Equality for primitive.
+
+Definition type_rep_eq_prim_checker F τ ηs : type_checker_res :=
+  match grab_rep F τ with
+  | Some ρ =>
+      match has_rep_checker F τ ρ with
+      | inl () =>
+          match eval_rep_prim EmptyEnv ρ with
+          | Some ηs1 =>
+              if list_beq primitive primitive_beq ηs ηs1
+              then ok_term
+              else INR "uh primitives don't match?"
+          | None => INR "bad rep i think"
+          end
+      | err => err
+      end
+  | None => INR "um not valtype?"
+  end.
+
+Lemma type_rep_eq_prim_checker_correct :
+  ∀ F τ ηs, type_rep_eq_prim_checker F τ ηs = ok_term -> type_rep_eq_prim F τ ηs.
+Proof.
+  intros.
+  unfold type_rep_eq_prim_checker in H.
+  repeat my_auto3.
+  apply has_rep_checker_correct in HMatch0. rename l into ηs1.
+  exists r. split; auto.
+  (* give some theorems about list_beq, this is obvious *)
+  admit.
+Admitted.
+
+(* NOTE: not a bit of confusing terminology. size_beq is actual equality.
+ size_eq_checker will be about it evalling to the same n *)
+
+Definition size_eq_checker σ1 σ2 : type_checker_res :=
+  match eval_size EmptyEnv σ1 with
+  | Some n1 =>
+      match eval_size EmptyEnv σ2 with
+      | Some n2 =>
+          if n1 =? n2
+          then ok_term
+          else INR "unequal sizes"
+      | None => INR "bad size"
+      end
+  | None => INR "bad size"
+  end.
+
+Lemma size_eq_checker_correct :
+  ∀ σ1 σ2, size_eq_checker σ1 σ2 = ok_term -> size_eq σ1 σ2.
+Proof.
+  intros. unfold size_eq_checker in *.
+  repeat my_auto3.
+  apply Nat.eqb_eq in HMatch1; subst.
+  econstructor; [apply HMatch | apply HMatch0].
+Qed.
+
+Definition size_leq_checker σ1 σ2 : type_checker_res :=
+  match eval_size EmptyEnv σ1 with
+  | Some n1 =>
+      match eval_size EmptyEnv σ2 with
+      | Some n2 =>
+          if n1 <? n2
+          then ok_term
+          else INR "unequal sizes"
+      | None => INR "bad size"
+      end
+  | None => INR "bad size"
+  end.
+
+Lemma size_leq_checker_correct :
+  ∀ σ1 σ2, size_leq_checker σ1 σ2 = ok_term -> size_leq σ1 σ2.
+Proof. (* easy *) Admitted.
+
+Definition type_size_eq_checker F τ1 τ2 : type_checker_res :=
+  match grab_size F τ1 with
+  | Some σ1 =>
+      match grab_size F τ2 with
+      | Some σ2 =>
+          match has_size_checker F τ1 σ1 with
+          | inl () =>
+              match has_size_checker F τ2 σ2 with
+              | inl () => size_eq_checker σ1 σ2
+              | err => err
+              end
+          | err => err
+          end
+      | None => INR "bad type for size"
+      end
+  | None => INR "bad type for size"
+  end.
+
+Lemma type_size_eq_checker_correct :
+  ∀ F τ1 τ2, type_size_eq_checker F τ1 τ2 = ok_term -> type_size_eq F τ1 τ2.
+Proof.
+  intros. unfold type_size_eq_checker in H.
+  repeat my_auto3.
+  apply has_size_checker_correct in HMatch1, HMatch3.
+  apply size_eq_checker_correct in H.
+  exists s, s0. split; auto.
+Qed.
+
+Definition grab_copyability F τ : option copyability :=
+  match grab_kind F τ with
+  | Some (VALTYPE _ χ _) => Some χ
+  | _ => None
+  end.
+
+Definition grab_dropability F τ : option dropability :=
+  match grab_kind F τ with
+  | Some (VALTYPE _ _ δ) => Some δ
+  | Some (MEMTYPE _ δ) => Some δ
+  | None => None
+  end.
+
+Definition has_copyability_checker F τ χ : type_checker_res :=
+  match grab_rep F τ with
+  | Some ρ => has_kind_checker F τ (VALTYPE ρ χ ImDrop)
+  | None => INR "not valtype"
+  end.
+
+Lemma has_copyability_checker_correct :
+  ∀ F τ χ, has_copyability_checker F τ χ = ok_term -> has_copyability F τ χ.
+Proof.
+  intros; unfold has_copyability_checker in *.
+  repeat my_auto3.
+  apply has_kind_checker_correct in H.
+  apply (CopyVALTYPE _ _ r _ ImDrop); auto.
+Qed.
+
+Definition has_dropability_checker F τ δ : type_checker_res :=
+  match grab_kind F τ with
+  | Some κ =>
+      match κ with
+      | VALTYPE ρ _ _ => has_kind_checker F τ (VALTYPE ρ ImCopy δ)
+      | MEMTYPE σ _ => has_kind_checker F τ (MEMTYPE σ δ)
+      end
+  | None => INR "bad kind"
+  end.
+
+Lemma has_dropability_checker_correct :
+  ∀ F τ δ, has_dropability_checker F τ δ = ok_term -> has_dropability F τ δ.
+Proof.
+  unfold has_dropability_checker; intros. repeat my_auto3; apply has_kind_checker_correct in H.
+  - by apply (DropVALTYPE _ _ r ImCopy _).
+  - by apply (DropMEMTYPE _ _ s _).
+Qed.
+
+
+
+(* Resolves path, and some other more complicated stuff before has_instruction_type *)
+
+Fixpoint get_list_of_reps (σs : list size) : option (list representation) :=
+  match σs with
+  | [] => Some []
+  | (RepS ρ) :: σss =>
+      match get_list_of_reps σss with
+      | Some ρs => Some (ρ :: ρs)
+      | None => None
+      end
+  | _ => None
+  end.
+
+Lemma get_list_of_reps_matches_map :
+  (∀ σs ρs, get_list_of_reps σs = Some ρs <-> σs = (map RepS ρs)).
+Proof.
+  split; intros.
+  - generalize dependent ρs.
+    induction σs.
+    + intros. simpl in H. inversion H; subst; simpl; auto.
+    + intros.
+      simpl in H.
+      repeat my_auto3. subst.
+      specialize (IHσs l). specialize (IHσs eq_refl).
+      subst; auto.
+  - generalize dependent ρs.
+    induction σs.
+    + intros. simpl in *.
+      symmetry in H; apply map_eq_nil in H.
+      by subst.
+    + intros; simpl in *.
+      symmetry in H.
+      destruct ρs; [simpl in H; inversion H |].
+      rewrite map_cons in H.
+      inversion H; subst.
+      specialize (IHσs ρs eq_refl).
+      by rewrite IHσs.
+Qed.
+
+
+Scheme Equality for num_type.
+
+Lemma num_type_eq_convert :
+  ∀ nt1 nt2, num_type_beq nt1 nt2 = true <-> nt1 = nt2.
+Proof. Admitted.
+
+(* type beq. Oh boy. Let's go. *)
+Fixpoint type_beq (τ1:type) (τ2:type) : bool :=
+  match τ1, τ2 with
+  | VarT i1, VarT i2 => i1 =? i2
+  | I31T κ1, I31T κ2 => kind_beq κ1 κ2
+  | NumT κ1 nt1, NumT κ2 nt2 => andb (kind_beq κ1 κ2) (num_type_beq nt1 nt2)
+  | SumT κ1 τs1, SumT κ2 τs2
+  | VariantT κ1 τs1, VariantT κ2 τs2
+  | ProdT κ1 τs1, ProdT κ2 τs2
+  | StructT κ1 τs1, StructT κ2 τs2 =>
+      andb (kind_beq κ1 κ2) (list_beq type type_beq τs1 τs2)
+  | RefT κ1 m1 τ1, RefT κ2 m2 τ2 =>
+      andb (andb (kind_beq κ1 κ2) (memory_beq m1 m2)) (type_beq τ1 τ2)
+  | CodeRefT κ1 ft1, CodeRefT κ2 ft2 =>
+      andb (kind_beq κ1 κ2) (function_type_beq ft1 ft2)
+  | SerT κ1 t1, SerT κ2 t2 => andb (kind_beq κ1 κ2) (type_beq t1 t2)
+  | PlugT κ1 ρ1, PlugT κ2 ρ2 => andb (kind_beq κ1 κ2) (representation_beq ρ1 ρ2)
+  | SpanT κ1 σ1, SpanT κ2 σ2 => andb (kind_beq κ1 κ2) (size_beq σ1 σ2)
+  | RecT κ1 t1, RecT κ2 t2
+  | ExistsMemT κ1 t1, ExistsMemT κ2 t2
+  | ExistsRepT κ1 t1, ExistsRepT κ2 t2
+  | ExistsSizeT κ1 t1, ExistsSizeT κ2 t2 =>
+      andb (kind_beq κ1 κ2) (type_beq t1 t2)
+  | ExistsTypeT κ11 κ12 t1, ExistsTypeT κ21 κ22 t2 =>
+      andb (andb (kind_beq κ11 κ21) (kind_beq κ12 κ22)) (type_beq t1 t2)
+  | _, _ => false
+  end
+with function_type_beq (fτ1:function_type) (fτ2:function_type) : bool :=
+  match fτ1, fτ2 with
+  | MonoFunT τs11 τs12, MonoFunT τs21 τs22 =>
+      andb (list_beq type type_beq τs11 τs21) (list_beq type type_beq τs12 τs22)
+  | ForallMemT ft1, ForallMemT ft2
+  | ForallRepT ft1, ForallRepT ft2
+  | ForallSizeT ft1, ForallSizeT ft2 => function_type_beq ft1 ft2
+  | ForallTypeT κ1 ft1, ForallTypeT κ2 ft2 =>
+      andb (kind_beq κ1 κ2) (function_type_beq ft1 ft2)
+  | _, _ => false
+  end.
+
+
+
+
+
+(* I should prove these eventually. Mainly to convince myself that
+list_beq will do what I want it to do. Although I think it's just fine.
+
+ TODO *)
+Lemma type_eq_convert :
+  ∀ τ1 τ2, type_beq τ1 τ2 = true <-> τ1 = τ2.
+Proof. Admitted.
+
+Lemma function_type_eq_convert :
+  ∀ ft1 ft2, function_type_beq ft1 ft2 = true <-> ft1 = ft2.
+Proof. Admitted.
+
+Ltac my_auto3_5 :=
+  match goal with
+  | H: ((match ?key with |_=>_ end) = _) |- _ => destruct key eqn:?HMatch; try inversion H; simpl in *
+  | H:((if ?key then _ else _)=_) |- _ => destruct key eqn:?HMatch; try inversion H; simpl in *
+  | H: (kind_beq _ _ = true) |- _ => apply kind_eq_convert in H; subst; auto
+  | o:ok |- _ => stupid_unit o
+  | H: ok_term = ok_term |- _ => clear H
+  | H: (andb _ _ = true) |- _ => apply andb_prop in H; destruct H as [?H1 ?H2]
+  | H: (_ && _ = true) |- _ => apply andb_prop in H; destruct H as [?H1 ?H2]
+  | H: (_ =? _ = true) |- _ => apply Nat.eqb_eq in H; subst; auto
+  | H: true = false |- _ => inversion H
+  | H: false = true |- _ => inversion H
+  | H: (num_type_beq _ _ = true) |- _ => apply num_type_eq_convert in H; subst; auto
+  | H: (type_beq _ _ = true) |- _ => apply type_eq_convert in H; subst; auto
+  | H: (function_type_beq _ _ = true) |- _ => apply function_type_eq_convert in H; subst; auto
+  | H: (representation_beq _ _ = true) |- _ => apply representation_eq_convert in H; subst; auto
+  | H: (dropability_beq _ _ = true) |- _ => apply dropability_eq_convert in H; subst; auto
+  | H: (copyability_beq _ _ = true) |- _ => apply copyability_eq_convert in H; subst; auto
+  | H: (size_beq _ _ = true) |- _ => apply size_eq_convert in H; subst; auto
+  | H: (memory_beq _ _ = true) |- _ => apply memory_eq_convert in H; subst; auto
+  | H: (kind_ok_checker _ _ = inl ()) |- _ => apply kind_ok_checker_correct in H; auto
+  | H: (kind_ok_checker _ _ = ok_term) |- _ => apply kind_ok_checker_correct in H; auto
+  | H: (mem_ok_checker _ _ = inl ()) |- _ => apply mem_ok_checker_correct in H; auto
+  | H: (mem_ok_checker _ _ = ok_term) |- _ => apply mem_ok_checker_correct in H; auto
+  | H: (rep_ok_checker _ _ = inl ()) |- _ => apply rep_ok_checker_correct in H; auto
+  | H: (rep_ok_checker _ _ = ok_term) |- _ => apply rep_ok_checker_correct in H; auto
+  | H: (size_ok_checker _ _ = inl ()) |- _ => apply size_ok_checker_correct in H; auto
+  | H: (size_ok_checker _ _ = ok_term) |- _ => apply size_ok_checker_correct in H; auto
+  | H: (type_ok_checker _ _ = inl ()) |- _ => apply type_ok_checker_correct in H; auto
+  | H: (type_ok_checker _ _ = ok_term) |- _ => apply type_ok_checker_correct in H; auto
+  | H: (function_type_ok_checker _ _ = inl ()) |- _ => apply function_type_ok_checker_correct in H; auto
+  | H: (function_type_ok_checker _ _ = ok_term) |- _ => apply function_type_ok_checker_correct in H; auto
+  | H: (has_kind_checker _ _ _ = ok_term) |- _ => apply has_kind_checker_correct in H; auto
+  | H: (has_kind_checker _ _ _ = inl ()) |- _ => apply has_kind_checker_correct in H; auto
+  | H: (check_if_subkind _ _ = inl ()) |- _ =>
+      try( by (eapply check_if_subkind_works_with_has_kind; try constructor; auto))
+  | H: (check_if_subkind _ _ = ok_term) |- _ =>
+      try( by (eapply check_if_subkind_works_with_has_kind; try constructor; auto))
+  | H: (INR _ = ok_term) |- _ => inversion H
+  | H: (INR _ = inl ()) |- _ => inversion H
+end.
+
+(* This is an attempt without a double match for the sake of the proof later *)
+Fixpoint type_eq_checker (F:function_ctx) (τ1:type) (τ2:type) :type_checker_res :=
+  (* base cases *)
+  match τ1 with
+  | VarT _ =>
+      match τ2 with
+      | VarT _ => if type_beq τ1 τ2 then ok_term else INR "types not equal"
+      | _ => INR "types note equal"
+      end
+  | I31T _ =>
+      match τ2 with
+      | I31T _ => if type_beq τ1 τ2 then ok_term else INR "types not equal"
+      | _ => INR "types not equal"
+      end
+  | NumT _ _ =>
+      match τ2 with
+      | NumT _ _ => if type_beq τ1 τ2 then ok_term else INR "types not equal"
+      | _ => INR "types note equal"
+      end
+  | CodeRefT _ _ =>
+      match τ2 with
+      | CodeRefT _ _ => if type_beq τ1 τ2 then ok_term else INR "types not equal"
+      | _ => INR "types note equal"
+      end
+  | PlugT _ _ =>
+      match τ2 with
+      | PlugT _ _ => if type_beq τ1 τ2 then ok_term else INR "types not equal"
+      | _ => INR "types note equal"
+      end
+  | SpanT _ _ =>
+      match τ2 with
+      | SpanT _ _ => if type_beq τ1 τ2 then ok_term else INR "types not equal"
+      | _ => INR "types note equal"
+      end
+  (* Recursive cases *)
+  | SumT κ1 τs1 =>
+      match τ2 with
+      | SumT κ2 τs2 =>
+          if kind_beq κ1 κ2
+          then
+            match has_kind_checker F (SumT κ1 τs1) κ1 with
+            | inl () =>
+                if foldr2 (λ τ1, λ τ2, andb (check_ok_output (type_eq_checker F τ1 τ2))) true τs1 τs2
+                then ok_term
+                else INR "types not equal"
+            | err => err
+            end
+          else INR "types not equal"
+      | _ => INR "types not equal"
+      end
+  | VariantT κ1 τs1 =>
+      match τ2 with
+      | VariantT κ2 τs2 =>
+          if kind_beq κ1 κ2
+          then
+            match has_kind_checker F (VariantT κ1 τs1) κ1 with
+            | inl () =>
+                if foldr2 (λ τ1, λ τ2, andb (check_ok_output (type_eq_checker F τ1 τ2))) true τs1 τs2
+                then ok_term
+                else INR "types not equal"
+            | err => err
+            end
+          else INR "types not equal"
+      | _ => INR "types not equal"
+      end
+  | ProdT κ1 τs1 =>
+      match τ2 with
+      | ProdT κ2 τs2 =>
+          if kind_beq κ1 κ2
+          then
+            match has_kind_checker F (ProdT κ1 τs1) κ1 with
+            | inl () =>
+                if foldr2 (λ τ1, λ τ2, andb (check_ok_output (type_eq_checker F τ1 τ2))) true τs1 τs2
+                then ok_term
+                else INR "types not equal"
+            | err => err
+            end
+          else INR "types not equal"
+      | _ => INR "types not equal"
+      end
+  | RefT κ1 μ1 τ1 =>
+      match τ2 with
+      | RefT κ2 μ2 τ2 =>
+          if andb (kind_beq κ1 κ2) (memory_beq μ1 μ2)
+          then
+            match has_kind_checker F (RefT κ1 μ1 τ1) κ1 with
+            | inl () => type_eq_checker F τ1 τ2
+            | err => err
+            end
+          else INR "types not equal"
+      | _ => INR "types not equal"
+      end
+  | RecT κ1 τ1 =>
+      match τ2 with
+      | RecT κ2 τ2 =>
+          if kind_beq κ1 κ2
+          then
+            match has_kind_checker F (RecT κ1 τ1) κ1 with
+            | inl () => type_eq_checker F τ1 τ2
+            | err => err
+            end
+          else INR "types not equal"
+      | _ => INR "types not equal"
+      end
+  | ExistsMemT κ1 τ1 =>
+      match τ2 with
+      | ExistsMemT κ2 τ2 =>
+          if kind_beq κ1 κ2
+          then
+            match has_kind_checker F (ExistsMemT κ1 τ1) κ1 with
+            | inl () => type_eq_checker F τ1 τ2
+            | err => err
+            end
+          else INR "types not equal"
+      | _ => INR "types not equal"
+      end
+  | ExistsRepT κ1 τ1 =>
+      match τ2 with
+      | ExistsRepT κ2 τ2 =>
+          if kind_beq κ1 κ2
+          then
+            match has_kind_checker F (ExistsRepT κ1 τ1) κ1 with
+            | inl () => type_eq_checker F τ1 τ2
+            | err => err
+            end
+          else INR "types not equal"
+      | _ => INR "types not equal"
+      end
+  | ExistsSizeT κ1 τ1 =>
+      match τ2 with
+      | ExistsSizeT κ2 τ2 =>
+          if kind_beq κ1 κ2
+          then
+            match has_kind_checker F (ExistsSizeT κ1 τ1) κ1 with
+            | inl () => type_eq_checker F τ1 τ2
+            | err => err
+            end
+          else INR "types not equal"
+      | _ => INR "types not equal"
+      end
+  | ExistsTypeT κ1 κτ1 τ1 =>
+      match τ2 with
+      | ExistsTypeT κ2 κτ2 τ2 =>
+          if andb (kind_beq κ1 κ2) (kind_beq κτ1 κτ2)
+          then
+            match has_kind_checker F (ExistsTypeT κ1 κτ1 τ1) κ1 with
+            | inl () => type_eq_checker F τ1 τ2
+            | err => err
+            end
+          else INR "types not equal"
+      | _ => INR "types not equal"
+      end
+  | SerT κ1 τ1 =>
+      match τ2 with
+      | SerT κ2 τ2 =>
+          if kind_beq κ1 κ2
+          then
+            match has_kind_checker F (SerT κ1 τ1) κ1 with
+            | inl () => type_eq_checker F τ1 τ2
+            | err => err
+            end
+          else INR "types not equal"
+      | StructT κ2 τs2 =>
+          match τ1 with
+          | ProdT κp τs =>
+              if kind_beq κ1 κ2
+              then (* I now throw away κ' *)
+                match κ1 with
+                | MEMTYPE (ProdS σs) δ =>
+                    match get_list_of_reps σs with
+                    | Some ρs =>
+                        if foldr2
+                             (λ τ:type, λ ρ:representation,
+                                   andb (check_ok_output (has_kind_checker F τ (VALTYPE ρ ImCopy δ)))
+                             ) true τs ρs
+                        then (* now just check that τs' equal to the monstrosity *)
+                          if list_beq type type_beq τs2 ((zip_with (fun τ ρ => SerT (MEMTYPE (RepS ρ) δ) τ)) τs ρs)
+                          then ok_term
+                          else INR "types not_equal"
+                        else INR "types not equal"
+                    | None => INR "types not equal"
+                    end
+                | _ => INR "types not equal"
+                end
+              else INR "types not equal"
+
+          | _ => INR "types not equal"
+          end
+      | _ => INR "types not equal"
+      end
+  | StructT κ1 τs1 =>
+      match τ2 with
+      | StructT κ2 τs2 =>
+          if kind_beq κ1 κ2
+          then
+            match has_kind_checker F (StructT κ1 τs1) κ1 with
+            | inl () =>
+                if foldr2 (λ τ1, λ τ2, andb (check_ok_output (type_eq_checker F τ1 τ2))) true τs1 τs2
+                then ok_term
+                else INR "types not equal 1"
+            | err => err
+            end
+          else INR "types not equal 2"
+      | SerT κ2 τ2 =>
+          match τ2 with
+          | ProdT κp τs =>
+              if kind_beq κ2 κ1
+              then (* I now throw away κ' *)
+                match κ2 with
+                | MEMTYPE (ProdS σs) δ =>
+                    match get_list_of_reps σs with
+                    | Some ρs =>
+                        if foldr2
+                             (λ τ:type, λ ρ:representation,
+                                   andb (check_ok_output (has_kind_checker F τ (VALTYPE ρ ImCopy δ)))
+                             ) true τs ρs
+                        then (* now just check that τs' equal to the monstrosity *)
+                          if list_beq type type_beq τs1 ((zip_with (fun τ ρ => SerT (MEMTYPE (RepS ρ) δ) τ)) τs ρs)
+                          then ok_term
+                          else INR "types not_equal 3"
+                        else INR "types not equal 4"
+                    | None => INR "types not equal 5"
+                    end
+                | _ => INR "types not equal 6"
+                end
+              else INR "types not equal 7"
+          | _ => INR "types not equal 8"
+          end
+
+      | _ => INR "types not equal HERE 9"
+      end
+
+  end.
+
+(* I'm bad at everything so monomorphic *)
+Lemma list_eq_convert_type :
+  ∀ τs1 τs2, list_beq type type_beq τs1 τs2 = true <-> τs1 = τs2.
+Proof. Admitted.
+Lemma list_eq_convert_size :
+  ∀ τs1 τs2, list_beq size size_beq τs1 τs2 = true <-> τs1 = τs2.
+Proof. Admitted.
+
+
+(* NOTE: the reason this has such a weird set up is because this
+   is the only way I know how to use type_and_function_ind
+
+  also NOTE: this is written more verbosely than ideal due to
+  the automation slowing down a Lot without a bit of help.
+ *)
+Opaque has_kind_checker.
+
+Lemma type_eq_checker_correct_basic :
+  (∀ τ1,
+     (∀ τ2, ∀ F, type_eq_checker F τ1 τ2 = ok_term -> type_eq F τ1 τ2)
+  ) /\
+  (∀ ft:function_type, True).
+Proof.
+  apply type_and_function_ind; auto; intros; destruct τ2.
+  (* the goal of this big guy: filter all obvious ones. Does not include "obvious" Ser *)
+  all:
+    match goal with
+    | |- (type_eq _ (VarT _) (VarT _)) => simpl in H; repeat my_auto3_5; apply TEqRefl
+    | |- (type_eq _ (I31T _) (I31T _)) => simpl in H; repeat my_auto3_5; apply TEqRefl; auto
+    | |- (type_eq _ (NumT _ _) (NumT _ _)) => simpl in H; repeat my_auto3_5; apply TEqRefl; repeat my_auto3_5
+    | |- (type_eq _ (SumT _ _) (SumT _ _)) => idtac
+    | |- (type_eq _ (VariantT _ _) (VariantT _ _)) => idtac
+    | |- (type_eq _ (ProdT _ _) (ProdT _ _)) => idtac
+    | |- (type_eq _ (StructT _ _) (StructT _ _)) => idtac
+    | |- (type_eq _ (RefT _ _ _) (RefT _ _ _)) =>
+        simpl in H0; repeat my_auto3_5; apply H in H0; apply TEqRef; auto
+    | |- (type_eq _ (CodeRefT _ _) (CodeRefT _ _)) => simpl in *; repeat my_auto3_5; apply TEqRefl; auto
+    | |- (type_eq _ (SerT _ _) (SerT _ _)) =>
+        simpl in H0; repeat my_auto3_5; apply TEqSer; auto
+    | |- (type_eq _ (StructT _ _) (SerT _ _)) => idtac
+    | |- (type_eq _ (SerT _ _) (StructT _ _)) => idtac
+    | |- (type_eq _ (SerT _ _) _) => simpl in H0; my_auto3_5
+    | |- (type_eq _ (PlugT _ _) (PlugT _ _)) => simpl in *; repeat my_auto3_5; apply TEqRefl; auto
+    | |- (type_eq _ (SpanT _ _) (SpanT _ _)) => simpl in *; repeat my_auto3_5; apply TEqRefl; auto
+    | |- (type_eq _ (RecT _ _) (RecT _ _)) =>
+        simpl in H0; repeat my_auto3_5; apply H in H0; apply TEqRec; auto
+    | |- (type_eq _ (ExistsMemT _ _) (ExistsMemT _ _)) =>
+        simpl in H0; repeat my_auto3_5; apply H in H0; apply TEqExMem; auto
+    | |- (type_eq _ (ExistsRepT _ _) (ExistsRepT _ _)) =>
+        simpl in H0; repeat my_auto3_5; apply H in H0; apply TEqExRep; auto
+    | |- (type_eq _ (ExistsSizeT _ _) (ExistsSizeT _ _)) =>
+        simpl in H0; repeat my_auto3_5; apply H in H0; apply TEqExSize; auto
+    | |- (type_eq _ (ExistsTypeT _ _ _) (ExistsTypeT _ _ _)) =>
+        simpl in H0; repeat my_auto3_5; apply H in H0; apply TEqExType; auto
+    | _ => simpl in *; my_auto3_5
+    end.
+
+  all: idtac. (* this is here because doom emacs despises the match goal above *)
+
+  (* ser struct case *)
+  6: {
+    simpl in H0. destruct t; simpl in H0; repeat my_auto3_5.
+    apply get_list_of_reps_matches_map in HMatch2; subst.
+    apply list_eq_convert_type in HMatch4; subst.
+    apply list_eq_convert_size in H1; subst.
+    apply (TEqSerProd _ _ l2 ImCopy d0 _).
+    (* this then relies on some foldr2 lemmas *)
+    admit.
+  }
+  (* struct ser case *)
+  5: {
+
+    simpl in H0. destruct τ2; simpl in H0; repeat my_auto3_5.
+    apply get_list_of_reps_matches_map in HMatch2; subst.
+    apply list_eq_convert_type in HMatch4; subst.
+    apply list_eq_convert_size in H1; subst.
+    apply TEqSym.
+    apply (TEqSerProd _ _ l1 ImCopy d0 _).
+    (* this then relies on some foldr2 lemmas *)
+    admit.
+
+  }
+  (* All the rest of are foldr2 lemma reliant, so *)
+  all: admit.
+
+Admitted.
+
+
+Lemma type_eq_checker_correct :
+  ∀ F τ1 τ2, type_eq_checker F τ1 τ2 = ok_term -> type_eq F τ1 τ2.
+Proof.
+  pose proof type_eq_checker_correct_basic.
+  destruct H as [H1 H2].
+  intros.
+  specialize (H1 τ1).
+  auto.
+Qed.
+
+
+Definition path_result_beq (pres1 pres2:path_result) : bool :=
+  andb (andb (list_beq type type_beq pres1.(pr_prefix) pres2.(pr_prefix))
+             (type_beq pres1.(pr_target) pres2.(pr_target)))
+             (type_beq pres1.(pr_replaced) pres2.(pr_replaced)).
+
+Lemma path_result_eq_convert :
+  ∀ pres1 pres2, path_result_beq pres1 pres2 = true <-> pres1 = pres2.
+Proof.
+  split; intros.
+  - unfold path_result_beq in H.
+    repeat my_auto3_5.
+    apply list_eq_convert_type in H1.
+    destruct pres1, pres2.
+    simpl in *. subst.
+    auto.
+  - destruct pres1, pres2.
+    inversion H; subst.
+    unfold path_result_beq. simpl.
+    apply andb_true_intro. split; [apply andb_true_intro; split |].
+    + apply list_eq_convert_type. auto.
+    + apply type_eq_convert; auto.
+    + apply type_eq_convert; auto.
+Qed.
+
+Fixpoint resolves_path_checker
+  (τ:type) (p:path) (oτ:option type) (pres:path_result) : type_checker_res :=
+  match p with
+  | [] =>
+      match oτ with
+      | Some τ' =>
+          if path_result_beq pres (Build_path_result [] τ τ')
+          then ok_term
+          else INR "does not resolve path"
+      | None =>
+          if path_result_beq pres (Build_path_result [] τ τ)
+          then ok_term
+          else INR "does not resolve path"
+      end
+  | i :: p => (* this is INCORRECT but temporary to allow for proving base case TODO *)
+      match τ with
+      | StructT κ τs_full => resolves_path_checker τ p oτ pres
+      | _ => INR "does not resolves path"
+      end
+  end.
+
+Lemma resolves_path_checker_correct_basic :
+  ∀ p τ oτ pres, resolves_path_checker τ p oτ pres = ok_term -> resolves_path τ p oτ pres.
+Proof.
+  intros p.
+  induction p.
+  - intros. unfold resolves_path_checker in H.
+    destruct oτ; repeat my_auto3_5; apply path_result_eq_convert in HMatch; subst.
+    + apply PathNilSome.
+    + apply PathNilNone.
+  -
+
+Admitted.
+
+Lemma resolves_path_checker_correct :
+  ∀ τ p oτ pres, resolves_path_checker τ p oτ pres = ok_term -> resolves_path τ p oτ pres.
+Proof. intros. apply resolves_path_checker_correct_basic. auto. Qed.
+
+
+Definition grab_inner_ft (ft:function_type) : option function_type :=
+  match ft with
+  | ForallMemT ϕ
+  | ForallRepT ϕ
+  | ForallSizeT ϕ
+  | ForallTypeT _ ϕ => Some ϕ
+  | MonoFunT _ _ => None
+  end.
+
+Ltac my_auto4 :=
+  match goal with
+  | H: ((match ?key with |_=>_ end) = _) |- _ => destruct key eqn:?HMatch; try inversion H; simpl in *
+  | H:((if ?key then _ else _)=_) |- _ => destruct key eqn:?HMatch; try inversion H; simpl in *
+  | H: (kind_beq _ _ = true) |- _ => apply kind_eq_convert in H; subst; auto
+  | o:ok |- _ => stupid_unit o
+  | H: ok_term = ok_term |- _ => clear H
+  | H: (andb _ _ = true) |- _ => apply andb_prop in H; destruct H as [?H1 ?H2]
+  | H: (_ && _ = true) |- _ => apply andb_prop in H; destruct H as [?H1 ?H2]
+  | H: true = false |- _ => inversion H
+  | H: false = true |- _ => inversion H
+  | H: (representation_beq _ _ = true) |- _ => apply representation_eq_convert in H; subst; auto
+  | H: (dropability_beq _ _ = true) |- _ => apply dropability_eq_convert in H; subst; auto
+  | H: (copyability_beq _ _ = true) |- _ => apply copyability_eq_convert in H; subst; auto
+  | H: (size_beq _ _ = true) |- _ => apply size_eq_convert in H; subst; auto
+  | H: (function_type_beq _ _ = true) |- _ => apply function_type_eq_convert in H; subst; auto
+  | H: (type_beq _ _ = true) |- _ => apply type_eq_convert in H; subst; auto
+  | H: (kind_ok_checker _ _ = inl ()) |- _ => apply kind_ok_checker_correct in H; auto
+  | H: (kind_ok_checker _ _ = ok_term) |- _ => apply kind_ok_checker_correct in H; auto
+  | H: (mem_ok_checker _ _ = inl ()) |- _ => apply mem_ok_checker_correct in H; auto
+  | H: (mem_ok_checker _ _ = ok_term) |- _ => apply mem_ok_checker_correct in H; auto
+  | H: (rep_ok_checker _ _ = inl ()) |- _ => apply rep_ok_checker_correct in H; auto
+  | H: (rep_ok_checker _ _ = ok_term) |- _ => apply rep_ok_checker_correct in H; auto
+  | H: (size_ok_checker _ _ = inl ()) |- _ => apply size_ok_checker_correct in H; auto
+  | H: (size_ok_checker _ _ = ok_term) |- _ => apply size_ok_checker_correct in H; auto
+  | H: (type_ok_checker _ _ = inl ()) |- _ => apply type_ok_checker_correct in H; auto
+  | H: (type_ok_checker _ _ = ok_term) |- _ => apply type_ok_checker_correct in H; auto
+  | H: (function_type_ok_checker _ _ = inl ()) |- _ => apply function_type_ok_checker_correct in H; auto
+  | H: (function_type_ok_checker _ _ = ok_term) |- _ => apply function_type_ok_checker_correct in H; auto
+  | H: (has_kind_checker _ _ _ = inl ()) |- _ => apply has_kind_checker_correct in H; auto
+  | H: (has_kind_checker _ _ _ = ok_term) |- _ => apply has_kind_checker_correct in H; auto
+  | H: (check_if_subkind _ _ = inl ()) |- _ =>
+      try( by (eapply check_if_subkind_works_with_has_kind; try constructor; auto))
+  | H: (check_if_subkind _ _ = ok_term) |- _ =>
+      try( by (eapply check_if_subkind_works_with_has_kind; try constructor; auto))
+end.
+
+Definition function_type_inst_checker
+  (F:function_ctx) (i:index) (ft1:function_type) (ft2:function_type) : type_checker_res :=
+  match i with
+  | MemI μ =>
+      match ft1 with
+      | ForallMemT ϕ =>
+          if function_type_beq ft2 (subst_function_type (unscoped.scons μ VarM) VarR VarS VarT ϕ)
+          then ok_term
+          else INR "something not matching in function type inst checker"
+      | _ => INR "bad function type inst"
+      end
+  | RepI ρ =>
+      match ft1 with
+      | ForallRepT ϕ =>
+          if function_type_beq ft2 (subst_function_type VarM (unscoped.scons ρ VarR) VarS VarT ϕ)
+          then ok_term
+          else INR "something not matching in function type inst checker"
+      | _ => INR "bad function type inst"
+      end
+  | SizeI σ =>
+      match ft1 with
+      | ForallSizeT ϕ =>
+          if function_type_beq ft2 (subst_function_type VarM VarR (unscoped.scons σ VarS) VarT ϕ)
+          then ok_term
+          else INR "something not matching in function type inst checker"
+      | _ => INR "bad function type inst"
+      end
+ | TypeI τ =>
+       match ft1 with
+      | ForallTypeT κ ϕ =>
+          match has_kind_checker F τ κ with
+          | inl () =>
+              if function_type_beq ft2 (subst_function_type VarM VarR VarS (unscoped.scons τ VarT) ϕ)
+              then ok_term
+              else INR "something not matching in function type inst checker"
+          | err => err
+          end
+      | _ => INR "bad function type inst"
+      end
+ end.
+
+
+Lemma function_type_inst_checker_correct :
+  ∀ F i ft1 ft2, function_type_inst_checker F i ft1 ft2 = ok_term -> function_type_inst F i ft1 ft2.
+Proof.
+  unfold function_type_inst_checker; intros.
+  repeat my_auto4.
+  all: constructor; auto.
+Qed.
+
+Definition grab_substed_ft F (ix:index) (ft1:function_type) : option function_type :=
+  match ix with
+  | MemI μ =>
+      match ft1 with
+      | ForallMemT ϕ => Some (subst_function_type (unscoped.scons μ VarM) VarR VarS VarT ϕ)
+      | _ => None
+      end
+  | RepI ρ =>
+      match ft1 with
+      | ForallRepT ϕ => Some (subst_function_type VarM (unscoped.scons ρ VarR) VarS VarT ϕ)
+      | _ => None
+      end
+  | SizeI σ =>
+      match ft1 with
+      | ForallSizeT ϕ => Some (subst_function_type VarM VarR (unscoped.scons σ VarS) VarT ϕ)
+      | _ => None
+      end
+ | TypeI τ =>
+       match ft1 with
+      | ForallTypeT κ ϕ =>
+          match has_kind_checker F τ κ with
+          | inl () => Some (subst_function_type VarM VarR VarS (unscoped.scons τ VarT) ϕ)
+          | _ => None
+          end
+      | _ => None
+      end
+  end.
+
+Fixpoint function_type_insts_checker
+      (F:function_ctx) (iss:list index) (ft1:function_type) (ft2:function_type) : type_checker_res :=
+  match iss with
+  | [] =>
+      if function_type_beq ft1 ft2
+      then ok_term
+      else INR "not equal in function_type_insts_checker"
+  | ix :: ixs =>
+      match grab_substed_ft F ix ft1 with
+      | Some ftinner =>
+          match function_type_inst_checker F ix ft1 ftinner with
+          | inl () => function_type_insts_checker F ixs ftinner ft2
+          | err => err
+          end
+      | None => INR "can't find ϕ' for FTCons"
+      end
+  end.
+
+Lemma function_type_insts_checker_correct :
+  ∀ F iss ft1 ft2, function_type_insts_checker F iss ft1 ft2 = ok_term ->
+                   function_type_insts F iss ft1 ft2.
+Proof.
+  intros F iss.
+  induction iss; intros; unfold function_type_insts_checker in H; repeat my_auto4.
+  - constructor.
+  - apply function_type_inst_checker_correct in HMatch0.
+    apply (FTCons _ _ f _ _ _); auto.
+Qed.
+
+
+(* TODO THIS IS SOMETHING I ACTUALLY AM UNSURE HOW TO DO *)
+Definition packed_existential_checker (F:function_ctx) (τ1 τ2:type) : type_checker_res :=
+  match τ2 with
+  | ExistsMemT κ' τ' =>
+      match has_kind_checker F τ' κ' with
+      | inl () =>
+          if true (* TODO HOW DO I GET THE MU OUT OF THERE *)
+            (*list_beq τ1 (subst_type (unscoped.scons μ VarM) VarR VarS VarT τ')*)
+          then ok_term
+          else INR "bad packed existential"
+      | err => err
+      end
+  | ExistsRepT κ' τ' => INR "incomplete"
+  | ExistsSizeT κ' τ' => INR "incomplete"
+  | ExistsTypeT κ' κ τ' => INR "incomplete"
+  | _ => INR "trying to check existential type, but not existential"
+  end.
+
+Lemma packed_existential_checker_correct :
+  ∀ F τ1 τ2, packed_existential_checker F τ1 τ2 = ok_term -> packed_existential F τ1 τ2.
+Proof.
+
+Admitted.
+
+(* This one has the reverse list stuff which I'm unsure how to do exactly *)
+Definition unpacked_existential_checker
+ (F:function_ctx) (L1:local_ctx) (insts:list instruction) (instt : instruction_type) (L2:local_ctx)
+ (F':function_ctx) (L1':local_ctx) (insts':list instruction) (instt': instruction_type) (L2':local_ctx)
+  :=
+  INR "incomplete".
+
+Lemma unpacked_existential_checker_correct :
+  ∀ F L1 insts instt L2 F' L1' insts' instt' L2',
+    unpacked_existential_checker F L1 insts instt L2 F' L1' insts' instt' L2' = ok_term ->
+    unpacked_existential F L2 insts instt L2 F' L1' insts' instt' L2'.
+Proof. Admitted.
+
+Definition local_ctx_ok_checker (F:function_ctx) (L:local_ctx) : type_checker_res :=
+  if foldr2
+       (λ t:type, λ p:list primitive,
+             andb (check_ok_output (type_rep_eq_prim_checker F t p))
+       ) true L (F.(fc_locals))
+  then ok_term
+  else INR "local context not ok".
+Lemma local_ctx_ok_checker_correct :
+  ∀ F L, local_ctx_ok_checker F L = ok_term -> local_ctx_ok F L.
+Proof.
+  (* this will be some foldr2 lemmas *)
+Admitted.
+
+
+
+
+
+(* And from here on, we move onto has_instruction_type stuff *)
+Definition has_instruction_type_ok_checker F ψ L' : type_checker_res :=
+  match has_mono_rep_instr_checker F ψ with
+  | inl () => local_ctx_ok_checker F L'
+  | err => err
+  end.
+Lemma has_instruction_type_ok_checker_correct :
+  ∀ F ψ L', has_instruction_type_ok_checker F ψ L' = ok_term -> has_instruction_type_ok F ψ L'.
+Proof.
+  intros. unfold has_instruction_type_ok_checker in H.
+  repeat my_auto3.
+  apply has_mono_rep_instr_checker_correct in HMatch.
+  clear H1 H2.
+  apply local_ctx_ok_checker_correct in H.
+  constructor; auto.
+Qed.
+
+
+(* NOTE: the reason I do InstrT [a] [b] for most of these is to speed up
+   the automation in the proof. Using the if then else is faster than
+   a match.
+   It also allows me to use the type functions/variables, (like type_i32)
+   rather than fully spelling out the type.
+ *)
+Definition has_instruction_type_cvt_checker cop ψ : type_checker_res :=
+  match cop with
+  | CWrap =>
+      match ψ with
+      | InstrT [a] [b] =>
+          if andb (type_beq a type_i64) (type_beq b type_i32)
+          then ok_term
+          else INR "incorrect cvt instruction type"
+      | _ => INR "incorrect cvt instruction type"
+      end
+  | CExtend _ =>
+      match ψ with
+      | InstrT [a] [b] =>
+          if andb (type_beq a type_i32) (type_beq b type_i64)
+          then ok_term
+          else INR "incorrect cvt instruction type"
+      | _ => INR "incorrect cvt instruction type"
+      end
+  | CTrunc vf vi _ =>
+      match ψ with
+      | InstrT [a] [b] =>
+          if andb (type_beq a (float_type_type vf)) (type_beq b (int_type_type vi))
+          then ok_term
+          else INR "incorrect cvt instruction type"
+      | _ => INR "incorrect cvt instruction type"
+      end
+  | CDemote =>
+      match ψ with
+      | InstrT [a] [b] =>
+          if andb (type_beq a type_f64) (type_beq b type_f32)
+          then ok_term
+          else INR "incorrect cvt instruction type"
+      | _ => INR "incorrect cvt instruction type"
+      end
+  | CPromote =>
+      match ψ with
+      | InstrT [a] [b] =>
+          if andb (type_beq a type_f32) (type_beq b type_f64)
+          then ok_term
+          else INR "incorrect cvt instruction type"
+      | _ => INR "incorrect cvt instruction type"
+      end
+  | CConvert vf vi _ =>
+      match ψ with
+      | InstrT [a] [b] =>
+          if andb (type_beq a (int_type_type vf)) (type_beq b (float_type_type vi))
+          then ok_term
+          else INR "incorrect cvt instruction type"
+      | _ => INR "incorrect cvt instruction type"
+      end
+  | CReinterpret (IntT I32T) =>
+      match ψ with
+      | InstrT [a] [b] =>
+          if andb (type_beq a type_i32) (type_beq b type_f32)
+          then ok_term
+          else INR "incorrect cvt instruction type"
+      | _ => INR "incorrect cvt instruction type"
+      end
+  | CReinterpret (IntT I64T) =>
+      match ψ with
+      | InstrT [a] [b] =>
+          if andb (type_beq a type_i64) (type_beq b type_f64)
+          then ok_term
+          else INR "incorrect cvt instruction type"
+      | _ => INR "incorrect cvt instruction type"
+      end
+  | CReinterpret (FloatT F32T) =>
+      match ψ with
+      | InstrT [a] [b] =>
+          if andb (type_beq a type_f32) (type_beq b type_i32)
+          then ok_term
+          else INR "incorrect cvt instruction type"
+      | _ => INR "incorrect cvt instruction type"
+      end
+  | CReinterpret (FloatT F64T) =>
+      match ψ with
+      | InstrT [a] [b] =>
+          if andb (type_beq a type_f64) (type_beq b type_i64)
+          then ok_term
+          else INR "incorrect cvt instruction type"
+      | _ => INR "incorrect cvt instruction type"
+      end
+  end.
+Lemma has_instruction_type_cvt_checker_correct :
+  ∀ cop ψ, has_instruction_type_cvt_checker cop ψ = ok_term -> has_instruction_type_cvt cop ψ.
+Proof.
+  intros. destruct cop; simpl in *; repeat my_auto4; subst; constructor.
+Qed.
+
+Definition has_instruction_type_num_checker ni ψ :=
+  match ni with
+  | IInt1 vi _ =>
+      match ψ with
+      | InstrT [a] [b] =>
+          if andb (type_beq a (int_type_type vi)) (type_beq b (int_type_type vi))
+          then ok_term
+          else INR "incorrect num instruction type[<35;19;60M]"
+      | _ => INR "incorrect num instruction type"
+      end
+  | IInt2 vi _ =>
+      match ψ with
+      | InstrT [a1; a2] [b] =>
+          if andb (andb (type_beq a1 (int_type_type vi)) (type_beq a2 (int_type_type vi)))
+                  (type_beq b (int_type_type vi))
+          then ok_term
+          else INR "incorrect num instruction type[<35;19;60M]"
+      | _ => INR "incorrect num instruction type"
+      end
+  | IIntTest vi _ =>
+      match ψ with
+      | InstrT [a] [b] =>
+          if andb (type_beq a (int_type_type vi)) (type_beq b type_i32)
+          then ok_term
+          else INR "incorrect num instruction type[<35;19;60M]"
+      | _ => INR "incorrect num instruction type"
+      end
+  | IIntRel vi _ =>
+      match ψ with
+      | InstrT [a1; a2] [b] =>
+          if andb (andb (type_beq a1 (int_type_type vi)) (type_beq a2 (int_type_type vi)))
+                  (type_beq b type_i32)
+          then ok_term
+          else INR "incorrect num instruction type[<35;19;60M]"
+      | _ => INR "incorrect num instruction type"
+      end
+  | IFloat1 vi _ =>
+      match ψ with
+      | InstrT [a] [b] =>
+          if andb (type_beq a (float_type_type vi)) (type_beq b (float_type_type vi))
+          then ok_term
+          else INR "incorrect num instruction type[<35;19;60M]"
+      | _ => INR "incorrect num instruction type"
+      end
+  | IFloat2 vi _ =>
+      match ψ with
+      | InstrT [a1; a2] [b] =>
+          if andb (andb (type_beq a1 (float_type_type vi)) (type_beq a2 (float_type_type vi)))
+                  (type_beq b (float_type_type vi))
+          then ok_term
+          else INR "incorrect num instruction type[<35;19;60M]"
+      | _ => INR "incorrect num instruction type"
+      end
+  | IFloatRel vi _ =>
+      match ψ with
+      | InstrT [a1; a2] [b] =>
+          if andb (andb (type_beq a1 (float_type_type vi)) (type_beq a2 (float_type_type vi)))
+                  (type_beq b type_i32)
+          then ok_term
+          else INR "incorrect num instruction type[<35;19;60M]"
+      | _ => INR "incorrect num instruction type"
+      end
+  | ICvt op => has_instruction_type_cvt_checker op ψ
+  end.
+Lemma has_instruction_type_num_checker_correct :
+  ∀ ni ψ, has_instruction_type_num_checker ni ψ = ok_term -> has_instruction_type_num ni ψ.
+Proof.
+  intros. destruct ni; simpl in *; repeat my_auto4; subst; try constructor.
+  apply has_instruction_type_cvt_checker_correct in H; auto.
+Qed.
+
+(* You know all the previous should have instead been using an instruction_type_beq. Oops.*)
+Definition instruction_type_beq (inst1 inst2:instruction_type) : bool :=
+  match inst1, inst2 with
+  | InstrT τs11 τs12, InstrT τs21 τs22 =>
+      andb (list_beq type type_beq τs11 τs21) (list_beq type type_beq τs12 τs22)
+  end.
+Lemma instruction_type_eq_convert :
+  ∀ inst1 inst2, instruction_type_beq inst1 inst2 = true <-> inst1 = inst2.
+Proof.
+  split; intros; destruct inst1, inst2; unfold instruction_type_beq in *; simpl in *.
+  - repeat my_auto3_5. apply list_eq_convert_type in H1, H2. subst; auto.
+  - inversion H; subst.
+    apply andb_true_intro; split; apply list_eq_convert_type; auto.
+Qed.
+
+About local_ctx.
+Definition local_ctx_beq (L L':local_ctx) : bool := list_beq type type_beq L L'.
+Lemma local_ctx_eq_convert :
+  ∀ L L', local_ctx_beq L L' = true <-> L = L'.
+Proof.
+  split; intros; unfold local_ctx_beq in *.
+  - apply list_eq_convert_type in H; subst; auto.
+  - subst; apply list_eq_convert_type; auto.
+Qed.
+
+(* I'm going to do this really stupidly *)
+Definition has_num_type_type (τ:type) : bool :=
+  orb (orb (type_beq τ (NumT (VALTYPE (AtomR I32R) ImCopy ImDrop) (IntT I32T)))
+           (type_beq τ (NumT (VALTYPE (AtomR I64R) ImCopy ImDrop) (IntT I64T))))
+      (orb (type_beq τ (NumT (VALTYPE (AtomR F32R) ImCopy ImDrop) (FloatT F32T)))
+           (type_beq τ (NumT (VALTYPE (AtomR F64R) ImCopy ImDrop) (FloatT F64T)))).
+Lemma has_num_type_type_correct :
+  ∀ τ, has_num_type_type τ = true <-> (∃ ν, τ = num_type_type ν).
+Proof.
+  split; intros; unfold has_num_type_type in *.
+  - apply orb_true_iff in H; destruct H as [H | H]; apply orb_true_iff in H; destruct H as [H | H];
+    apply type_eq_convert in H; subst.
+    + exists (IntT I32T); auto.
+    + exists (IntT I64T); auto.
+    + exists (FloatT F32T); auto.
+    + exists (FloatT F64T); auto.
+  - repeat rewrite orb_true_iff.
+    destruct H as [ν H].
+    destruct ν; [destruct i | destruct f].
+    + left; left. by apply type_eq_convert.
+    + left; right. by apply type_eq_convert.
+    + right; left. by apply type_eq_convert.
+    + right; right. by apply type_eq_convert.
+Qed.
+
+Fixpoint check_recursion_single_inner (inst:instruction) : bool :=
+  let fix check_recursion_list_inner insts : bool :=
+    match insts with
+    | [] => true
+    | e :: es => andb (check_recursion_single_inner e) (check_recursion_list_inner es)
+    end
+  in
+  match inst with
+  | IUnreachable _ => false
+  | IBlock _ _ es => check_recursion_list_inner es
+  | _ => true
+  end.
+
+Fail Fixpoint check_recursion_single_outer (inst:instruction) : bool :=
+  match inst with
+  | IUnreachable _ => false
+  | IBlock _ _ es => check_recursion_list_outer es
+  | _ => true
+  end
+with check_recursion_list_outer insts : bool :=
+  match insts with
+  | [] => true
+  | e :: es => andb (check_recursion_single_outer e) (check_recursion_list_outer es)
+  end.
+
+
+Fixpoint split_list_all_last {A:Type} (l:list A) : option (list A * A) :=
+  match l with
+  | [] => None
+  | [a] => Some ([], a)
+  | h :: rest =>
+      match split_list_all_last rest with
+      | Some (ll, last) => Some (h::ll, last)
+      | None => None
+      end
+  end.
+
+Lemma split_list_all_last_correct :
+  ∀ (A:Type) (l ls:list A) (last:A),
+    split_list_all_last l = Some (ls, last) -> l = ls ++ [last].
+Proof.
+  intros A l.
+  induction l.
+  - intros. simpl in H; inversion H.
+  - intros.
+    simpl in H.
+    destruct l.
+    + inversion H; subst.
+      by rewrite app_nil_l.
+    + my_auto4.
+      clear H1.
+      destruct p. inversion H. subst.
+      specialize (IHl l0 last eq_refl).
+      rewrite IHl. auto.
+Qed.
+
+Fixpoint list_suffix_helper (l1 l2: list type) (l1len l2len: nat) : option (list type) :=
+  if l1len =? l2len
+  then
+    if list_beq type type_beq l1 l2
+    then Some []
+    else None
+  else
+    match l1, l1len with
+    | h::rest, S n =>
+        match list_suffix_helper rest l2 n l2len with
+        | Some pr => Some (h::pr)
+        | None => None
+        end
+    | _, _ => None
+    end.
+
+Definition list_suffix l1 l2 : option (list type) :=
+  let l1len := Init.Datatypes.length l1 in
+  let l2len := Init.Datatypes.length l2 in
+  list_suffix_helper l1 l2 l1len l2len.
+
+Lemma list_suffix_correct :
+  ∀ lfull lpre lsuf,
+    lfull = lpre ++ lsuf -> list_suffix lfull lsuf = Some lpre.
+Proof.
+  intros lfull.
+  induction lfull.
+  - intros.
+    destruct lpre, lsuf; try inversion H.
+    auto.
+  - intros lprebig.
+    destruct lprebig as [ | a' lpre ].
+    + admit.
+    + intros.
+      inversion H; subst.
+      specialize (IHlfull lpre lsuf eq_refl).
+      (* yeah this is right *)
+      admit.
+Admitted.
+
+
+
+(* Will need a mutually recursive have_instruction_type too *)
+Fixpoint has_instruction_type_checker
+    (M:module_ctx) (F:function_ctx) (L:local_ctx)
+    (inst:instruction) (ψ:instruction_type) (L':local_ctx) {struct inst} : type_checker_res :=
+  let fix have_instruction_type_checker
+    (M:module_ctx) (F:function_ctx) (L:local_ctx)
+    (insts:list instruction) (ψ:instruction_type) (L':local_ctx) {struct insts} : type_checker_res :=
+    match insts with
+    | [] =>
+        if andb (instruction_type_beq ψ (InstrT [] [])) (local_ctx_beq L L')
+        then local_ctx_ok_checker F L
+        else INR "bad empty instructions type"
+    (*| [e] => has_instruction_type_checker M F L e ψ L'*)
+    | e :: es => (* NOTE THIS IS FUNDAMENTALLY INCORRECT!!! THIS IS TEMPORARY FOR CHECKING RECURSION *)
+        match have_instruction_type_checker M F L es ψ L' with
+        | inl () => has_instruction_type_checker M F L e ψ L'
+        | err => err
+        end
+    end
+  in
+
+  match inst with
+  (*  BASE CASES  *)
+  | INop ψ_inner =>
+      if andb (andb (instruction_type_beq ψ (InstrT [] []))
+           (instruction_type_beq ψ_inner (InstrT [] []))) (local_ctx_beq L L')
+      then has_instruction_type_ok_checker F ψ L
+      else INR "incorrect instruction type for nop"
+  | IUnreachable ψ_inner =>
+      if instruction_type_beq ψ ψ_inner
+      then has_instruction_type_ok_checker F ψ L'
+      else INR "incorrect instruction type for unreachable"
+  | ICopy ψ_inner =>
+      if andb (instruction_type_beq ψ ψ_inner) (local_ctx_beq L L')
+      then
+        match ψ with
+        | InstrT [τ] [τ1;τ2] =>
+            if andb (type_beq τ τ1) (type_beq τ1 τ2)
+            then
+              match has_copyability_checker F τ ExCopy with
+              | inl () => has_instruction_type_ok_checker F ψ L
+              | _ => INR "incorrect copyability for instruction type for copy"
+              end
+            else INR "incorrect instruction type for copy"
+        | _ => INR "incorrect instruction type for copy"
+        end
+      else INR "incorrect instruction type for copy"
+  | IDrop ψ_inner =>
+      if andb (instruction_type_beq ψ ψ_inner) (local_ctx_beq L L')
+      then
+        match ψ with
+        | InstrT [τ] [] => has_instruction_type_ok_checker F ψ L
+        | _ => INR "incorrect instruction type for drop"
+        end
+      else INR "incorrect instruction type for drop"
+  | INum ψ_inner e =>
+      if andb (instruction_type_beq ψ ψ_inner) (local_ctx_beq L L')
+      then
+        match has_instruction_type_num_checker e ψ with
+        | inl () => has_instruction_type_ok_checker F ψ L
+        | err => err
+        end
+      else INR "incorrect instruction type for num"
+  | INumConst ψ_inner n =>
+      if andb (instruction_type_beq ψ ψ_inner) (local_ctx_beq L L')
+      then
+        match ψ with
+        | InstrT [] [τ] =>
+            if has_num_type_type τ
+            then has_instruction_type_ok_checker F ψ L
+            else INR "incorrect instruction type for numconst"
+        | _ => INR "incorrect instruction type for numconst"
+        end
+      else INR "incorrect instruction type for numconst"
+  (* not base cases lmao *)
+  | IBlock ψ_inner L_inner es =>
+      if andb (instruction_type_beq ψ ψ_inner) (local_ctx_beq L' L_inner)
+      then (* this INCORRECT but just to check if the recursion goes through *)
+        match ψ with
+        | InstrT τs1 τs2 =>
+            match have_instruction_type_checker M (F <| fc_labels ::= cons (τs2, L') |>) L es ψ L' with
+            | inl () => has_instruction_type_ok_checker F ψ L'
+            | err => err
+            end
+        end
+      else INR "incorrect instruction type for block"
+  | ILoop ψ_inner es =>
+      if andb (instruction_type_beq ψ ψ_inner) (local_ctx_beq L L')
+      then
+        match ψ with
+        | InstrT τs1 τs2 =>
+            match have_instruction_type_checker M (F <| fc_labels ::= cons (τs1, L) |>) L es ψ L with
+            | inl () => has_instruction_type_ok_checker F ψ L
+            | err => err
+            end
+        end
+      else INR "incorrect instruction type for loop"
+  | IIte ψ_inner L_inner es1 es2 =>
+      if andb (instruction_type_beq ψ ψ_inner) (local_ctx_beq L_inner L')
+      then
+        match ψ with
+        | InstrT τs1_full τs2 =>
+            match split_list_all_last τs1_full with
+            | Some (τs1, τ) =>
+                if type_beq τ type_i32
+                then
+                  match have_instruction_type_checker M (F <| fc_labels ::= cons (τs2, L') |>) L
+                          es1 (InstrT τs1 τs2) L' with
+                  | inl () =>
+                      match have_instruction_type_checker M (F <| fc_labels ::= cons (τs2, L') |>) L
+                          es2 (InstrT τs1 τs2) L' with
+                      | inl () => has_instruction_type_ok_checker F ψ L'
+                      | err => err
+                      end
+                  | err => err
+                  end
+                else INR "instruction type for ite does not have i32"
+            | None => INR "instruction type for ite does not have i32"
+            end
+        end
+      else INR "incorrect instruction type for ite"
+  | IBr ψ_inner i =>
+      if instruction_type_beq ψ ψ_inner
+      then
+        match F.(fc_labels) !! i with
+        | Some (τs, L_inner) =>
+            if local_ctx_beq L_inner L
+            then (* okay now we have to ensure ts1_full is split correctly *)
+              match ψ with
+              | InstrT τs1_full τs2 =>
+                  match list_suffix τs1_full τs with
+                  | Some τs1 =>
+                      if true (* if all ImDrop TODO *)
+                      then has_instruction_type_ok_checker F ψ L'
+                      else INR "incorrect instruction type for br"
+                  | None => INR "incorrect instruction type for br"
+                  end
+              end
+            else INR "incorrect instruction type for br"
+        | None => INR "incorrect instruction type for br, something with fc labels"
+        end
+      else INR "incorrect instruction type for br"
+  | IReturn ψ_inner =>
+      if instruction_type_beq ψ ψ_inner
+      then
+        let τs := F.(fc_return) in
+        match ψ with
+        | InstrT τs1_full τs2 =>
+            match list_suffix τs1_full τs with
+            | Some τs1 =>
+                if true (* if all ImDrop TODO *)
+                then has_instruction_type_ok_checker F ψ L'
+                else INR "incorrect instruction type for return"
+            | None => INR "incorrect instruction type for return"
+            end
+        end
+      else INR "incorrect instruction type for return"
+  | ILocalGet ψ_inner i => (* note this is for both TLocalGetMove and TLocalGetCopy *)
+      if andb (instruction_type_beq ψ ψ_inner) (true)
+      then
+        match L !! i with
+        | Some τ =>
+            match ψ with
+            | InstrT [] [τ'] =>
+                if type_beq τ τ'
+                then
+                  match has_copyability_checker F τ ImCopy with (* decision point *)
+                  | inl () =>
+                      if local_ctx_beq L L'
+                      then has_instruction_type_ok_checker F ψ L
+                      else INR "incorrect instruction type for local get"
+                  | inr _ =>
+                      match F.(fc_locals) !! i with
+                      | Some ηs =>
+                          if local_ctx_beq L' (<[ i := type_plug_prim ηs ]> L)
+                          then has_instruction_type_ok_checker F ψ L'
+                          else INR "incorrect instruction type for local get"
+                      | None => INR "incorrect instruction type for local get"
+                      end
+                  end
+                else INR "incorrect instruction type for local get"
+            | InstrT _ _ => INR "incorrect instruction type for local get (shape not [] -> [τ])"
+            end
+        | None => INR "incorrect instruction type for local get (i not in local context)"
+        end
+      else INR "incorrect instruction type for local get"
+  | ICodeRef ψ_inner i =>
+      if andb (instruction_type_beq ψ ψ_inner) (local_ctx_beq L L')
+      then
+        match ψ with
+        | InstrT [] [τ'] =>
+            match M.(mc_table) !! i with
+            | Some ϕ =>
+                if type_beq τ' (CodeRefT (VALTYPE (AtomR I32R) ImCopy ImDrop) ϕ)
+                then has_instruction_type_ok_checker F ψ L
+                else INR "incorrect instruction type for coderef"
+            | None => INR "incorrect instruction type for coderef"
+            end
+        | InstrT _ _ => INR "incorrect instruction type for coderef (wrong shape)"
+        end
+      else INR "incorrect instruction type for coderef"
+  | IInst ψ_inner ix =>
+      if andb (instruction_type_beq ψ ψ_inner) (local_ctx_beq L L')
+      then
+        match ψ with
+        | InstrT [a] [b] =>
+            match a, b with
+            | CodeRefT κ ϕ, CodeRefT κ' ϕ' =>
+                if andb (kind_beq κ (VALTYPE (AtomR I32R) ImCopy ImDrop)) (kind_beq κ κ')
+                then
+                  match function_type_inst_checker F ix ϕ ϕ' with
+                  | inl () => has_instruction_type_ok_checker F ψ L
+                  | err => err
+                  end
+                else INR "incorrect instruction type for IInst"
+            | _, _ => INR "incorrect instruction type for IINst"
+            end
+        | _ => INR "incorrect instruction type for IInst (wrong shape)"
+        end
+      else INR "incorrect instruction type for IINst"
+  | ICall ψ_inner i ixs =>
+      if andb (instruction_type_beq ψ ψ_inner) (local_ctx_beq L L')
+      then
+        match ψ with
+        | InstrT τs1 τs2 =>
+            match M.(mc_functions) !! i with
+            | Some ϕ =>
+                match function_type_insts_checker F ixs ϕ (MonoFunT τs1 τs2) with
+                | inl () => has_instruction_type_ok_checker F ψ L
+                | err => err
+                end
+            | None => INR "incorrect instruction type for call"
+            end
+        end
+      else INR "incorrect instruction type for call"
+  | ICallIndirect ψ_inner =>
+      if andb (instruction_type_beq ψ ψ_inner) (local_ctx_beq L L')
+      then
+        match ψ with
+        | InstrT τs1_full τs2 =>
+            match split_list_all_last τs1_full with
+            | Some (τs1, τ) =>
+                if type_beq τ (CodeRefT (VALTYPE (AtomR I32R) ImCopy ImDrop) (MonoFunT τs1 τs2))
+                then has_instruction_type_ok_checker F ψ L
+                else INR "incorrect instruction type for call indirect"
+            | None => INR "incorrect instruction type for call indirect"
+            end
+        end
+      else INR "incorrect instruction type for call indirect"
+  | IInject ψ_inner i =>
+      if andb (instruction_type_beq ψ ψ_inner) (local_ctx_beq L L')
+      then
+        match ψ with
+        | InstrT [τ'] [a] =>
+            match a with
+            | SumT κ τs =>
+                match τs !! i with
+                | Some τ =>
+                    if type_beq τ' τ
+                    then has_instruction_type_ok_checker F ψ L
+                    else INR "incorrect instruction type for inject"
+                | None => INR "incorrect instruction type for inject"
+                end
+            | _ => INR "incorrect instruction type for inject (wrong shape)"
+            end
+        | _ => INR "incorrect instruction type for inject (wrong shape)"
+        end
+      else INR "incorrect instruction type for inject"
+  | IInjectNew ψ_inner i => INR "incomplete" (* TODO do i have smthn for zip_with already *)
+  | ICase ψ_inner L_inner ess => INR "incomplete"
+  | ICaseLoad ψ_inner cm L_inner ess => INR "incomplete"
+  | IGroup ψ_inner =>
+      if andb (instruction_type_beq ψ ψ_inner) (local_ctx_beq L L')
+      then
+        match ψ with
+        | InstrT τs [a] =>
+            match a with
+            | ProdT κ τs' =>
+                if list_beq type type_beq τs τs'
+                then has_instruction_type_ok_checker F ψ L
+                else INR "incorrect instruction type for group"
+            | _ => INR "incorrect instruction type for group (wrong shape)"
+            end
+        | _ => INR "incorrect instruction type for group (wrong shape)"
+        end
+      else INR "incorrect instruction type for group"
+  | IUngroup ψ_inner =>
+      if andb (instruction_type_beq ψ ψ_inner) (local_ctx_beq L L')
+      then
+        match ψ with
+        | InstrT [a] τs =>
+            match a with
+            | ProdT κ τs' =>
+                if list_beq type type_beq τs τs'
+                then has_instruction_type_ok_checker F ψ L
+                else INR "incorrect instruction type for ungroup"
+            | _ => INR "incorrect instruction type for ungroup (wrong shape)"
+            end
+        | _ => INR "incorrect instruction type for ungroup (wrong shape)"
+        end
+      else INR "incorrect instruction type for ungroup"
+  | IFold ψ_inner =>
+      if andb (instruction_type_beq ψ ψ_inner) (local_ctx_beq L L')
+      then
+        match ψ with
+        | InstrT [τ0] [a] =>
+            match a with
+            | RecT κ τ =>
+                if type_beq τ0 (subst_type VarM VarR VarS (unscoped.scons (RecT κ τ) VarT) τ)
+                then has_instruction_type_ok_checker F ψ L
+                else INR "incorrect instruction type for fold"
+            | _ => INR "incorrect instruction type for fold (wrong shape)"
+            end
+        | _ => INR "incorrect instruction type for fold (wrong shape)"
+        end
+      else INR "incorrect instruction type for fold"
+  | IUnfold ψ_inner =>
+      if andb (instruction_type_beq ψ ψ_inner) (local_ctx_beq L L')
+      then
+        match ψ with
+        | InstrT [a] [τ0] =>
+            match a with
+            | RecT κ τ =>
+                if type_beq τ0 (subst_type VarM VarR VarS (unscoped.scons (RecT κ τ) VarT) τ)
+                then has_instruction_type_ok_checker F ψ L
+                else INR "incorrect instruction type for unfold"
+            | _ => INR "incorrect instruction type for unfold (wrong shape)"
+            end
+        | _ => INR "incorrect instruction type for unfold (wrong shape)"
+        end
+      else INR "incorrect instruction type for unfold"
+  | IPack ψ_inner =>
+      if andb (instruction_type_beq ψ ψ_inner) (local_ctx_beq L L')
+      then
+        match ψ with
+        | InstrT [τ] [τ'] =>
+            match packed_existential_checker F τ τ' with
+            | inl () => has_instruction_type_ok_checker F ψ L
+            | err => err
+            end
+        | _ => INR "incorrect instruction type for pack"
+        end
+      else INR "incorrect instruction type for pack"
+  | IUnpack ψ_inner L_inner es => INR "incomplete"
+  | ITag ψ_inner =>
+      if andb (instruction_type_beq ψ ψ_inner) (local_ctx_beq L L')
+      then
+        match ψ with
+        | InstrT [a] [b] =>
+            if andb (type_beq a type_i32) (type_beq b type_i31)
+            then has_instruction_type_ok_checker F ψ L
+            else INR "incorrect instruction type for tag"
+        | _ => INR "incorrect instruction type for tag (wrong shape)"
+        end
+      else INR "incorrect instruction type for tag"
+  | IUntag ψ_inner =>
+      if andb (instruction_type_beq ψ ψ_inner) (local_ctx_beq L L')
+      then
+        match ψ with
+        | InstrT [b] [a] =>
+            if andb (type_beq a type_i32) (type_beq b type_i31)
+            then has_instruction_type_ok_checker F ψ L
+            else INR "incorrect instruction type for untag"
+        | _ => INR "incorrect instruction type for untag (wrong shape)"
+        end
+      else INR "incorrect instruction type for untag"
+  | ICast ψ_inner =>
+      if andb (instruction_type_beq ψ ψ_inner) (local_ctx_beq L L')
+      then
+        match ψ with
+        | InstrT [τ] [τ'] =>
+            match type_eq_checker F τ τ' with
+            | inl () => has_instruction_type_ok_checker F ψ L
+            | err => err
+            end
+        | _ => INR "incorrect instruction type for cast (wrong shape)"
+        end
+      else INR "incorrect instruction type for cast"
+  | INew ψ_inner =>
+      if andb (instruction_type_beq ψ ψ_inner) (local_ctx_beq L L')
+      then
+        match ψ with
+        | InstrT [τ] [a] =>
+            match a with
+            | RefT κ μ (SerT κser τ') =>
+                if type_beq τ τ'
+                then
+                  match mono_mem_checker μ with
+                  | inl () => has_instruction_type_ok_checker F ψ L
+                  | err => err
+                  end
+                else INR "incorrect instruction type for new"
+            | _ => INR "incorrect instruction type for new (wrong shape)"
+            end
+        | _ => INR "incorrect instruction type for new (wrong shape)"
+        end
+      else INR "incorrect instruction type for new"
+  | ILoad ψ_inner π cm => (* note this will be both TLoadCopy and TLoadMove *)
+      INR "incomplete"
+  | IStore ψ_inner π => (* note this will be both TStoreWeak and TStoreStrong *)
+      INR "incomplete"
+  | TSwap ψ_inner π =>
+      if andb (instruction_type_beq ψ ψ_inner) (local_ctx_beq L L')
+      then INR "incomplete"
+      else INR "incorrect instruction type for swap"
+  | _ => INR "incomplete"
+  end.
+(*
+with have_instruction_type_checker
+    (M:module_ctx) (F:function_ctx) (L:local_ctx)
+    (insts:list instruction) (ψ:instruction_type) (L':local_ctx) {struct insts} : type_checker_res :=
+  match insts with
+  | [] =>
+      if andb (instruction_type_beq ψ (InstrT [] [])) (local_ctx_beq L L')
+      then local_ctx_ok_checker F L
+      else INR "bad empty instructions type"
+  (*| [e] => has_instruction_type_checker M F L e ψ L'*)
+  | e :: es => (* NOTE THIS IS FUNDAMENTALLY INCORRECT!!! THIS IS TEMPORARY FOR STRUCTURE *)
+      match has_instruction_type_checker M F L e ψ L' with
+      | inl () => have_instruction_type_checker M F L es ψ L'
+      | err => err
+      end
+  end.
+  *)
+Ltac my_auto5 :=
+  match goal with
+  | H: ((match ?key with |_=>_ end) = _) |- _ => destruct key eqn:?HMatch; try inversion H; simpl in *
+  | H:((if ?key then _ else _)=_) |- _ => destruct key eqn:?HMatch; try inversion H; simpl in *
+  | H: (kind_beq _ _ = true) |- _ => apply kind_eq_convert in H; subst; auto
+  | o:ok |- _ => stupid_unit o
+  | H: ok_term = ok_term |- _ => clear H
+  | H: (andb _ _ = true) |- _ => apply andb_prop in H; destruct H as [?H1 ?H2]
+  | H: (_ && _ = true) |- _ => apply andb_prop in H; destruct H as [?H1 ?H2]
+  | H: true = false |- _ => inversion H
+  | H: false = true |- _ => inversion H
+  | H: (instruction_type_beq _ _ = true) |- _ => apply instruction_type_eq_convert in H; subst; auto
+  | H: (local_ctx_beq _ _ = true) |- _ => apply local_ctx_eq_convert in H; subst; auto
+  | H: (representation_beq _ _ = true) |- _ => apply representation_eq_convert in H; subst; auto
+  | H: (dropability_beq _ _ = true) |- _ => apply dropability_eq_convert in H; subst; auto
+  | H: (copyability_beq _ _ = true) |- _ => apply copyability_eq_convert in H; subst; auto
+  | H: (size_beq _ _ = true) |- _ => apply size_eq_convert in H; subst; auto
+  | H: (function_type_beq _ _ = true) |- _ => apply function_type_eq_convert in H; subst; auto
+  | H: (type_beq _ _ = true) |- _ => apply type_eq_convert in H; subst; auto
+  | H: (kind_ok_checker _ _ = inl ()) |- _ => apply kind_ok_checker_correct in H; auto
+  | H: (kind_ok_checker _ _ = ok_term) |- _ => apply kind_ok_checker_correct in H; auto
+  | H: (mem_ok_checker _ _ = inl ()) |- _ => apply mem_ok_checker_correct in H; auto
+  | H: (mem_ok_checker _ _ = ok_term) |- _ => apply mem_ok_checker_correct in H; auto
+  | H: (rep_ok_checker _ _ = inl ()) |- _ => apply rep_ok_checker_correct in H; auto
+  | H: (rep_ok_checker _ _ = ok_term) |- _ => apply rep_ok_checker_correct in H; auto
+  | H: (size_ok_checker _ _ = inl ()) |- _ => apply size_ok_checker_correct in H; auto
+  | H: (size_ok_checker _ _ = ok_term) |- _ => apply size_ok_checker_correct in H; auto
+  | H: (type_ok_checker _ _ = inl ()) |- _ => apply type_ok_checker_correct in H; auto
+  | H: (type_ok_checker _ _ = ok_term) |- _ => apply type_ok_checker_correct in H; auto
+  | H: (function_type_ok_checker _ _ = inl ()) |- _ => apply function_type_ok_checker_correct in H; auto
+  | H: (function_type_ok_checker _ _ = ok_term) |- _ => apply function_type_ok_checker_correct in H; auto
+  | H: (has_kind_checker _ _ _ = inl ()) |- _ => apply has_kind_checker_correct in H; auto
+  | H: (has_kind_checker _ _ _ = ok_term) |- _ => apply has_kind_checker_correct in H; auto
+  | H: (has_instruction_type_ok_checker _ _ _ = ok_term) |- _ => apply has_instruction_type_ok_checker_correct in H; auto
+  | H: (has_instruction_type_ok_checker _ _ _ = inl ()) |- _ => apply has_instruction_type_ok_checker_correct in H; auto
+  | H: (has_instruction_type_num_checker _ _ = ok_term) |- _ => apply has_instruction_type_num_checker_correct in H; auto
+  | H: (has_instruction_type_num_checker _ _ = inl ()) |- _ => apply has_instruction_type_num_checker_correct in H; auto
+  | H: (has_copyability_checker _ _ _ = ok_term) |- _ => apply has_copyability_checker_correct in H; auto
+  | H: (has_copyability_checker _ _ _ = inl ()) |- _ => apply has_copyability_checker_correct in H; auto
+  | H: (check_if_subkind _ _ = inl ()) |- _ =>
+      try( by (eapply check_if_subkind_works_with_has_kind; try constructor; auto))
+  | H: (check_if_subkind _ _ = ok_term) |- _ =>
+      try( by (eapply check_if_subkind_works_with_has_kind; try constructor; auto))
+end.
+
+
+Lemma has_instruction_type_checker_correct :
+  ∀ M F L inst ψ L',
+    has_instruction_type_checker M F L inst ψ L' = ok_term ->
+    has_instruction_type M F L inst ψ L'.
+Proof.
+  intros.
+  destruct inst.
+  - (* nop, using destruct inst, without have_instruction_type *)
+    unfold has_instruction_type_checker in H.
+    repeat my_auto5. by constructor.
+  - (* unreachable, using destruct inst, without have-instruction_type*)
+    unfold has_instruction_type_checker in H; repeat my_auto5; by constructor.
+  - (* copy, using destruct inst, without have_instruction_type *)
+    unfold has_instruction_type_checker in H; repeat my_auto5; by constructor.
+  - (* drop, using destruct inst, without have_instruction_type *)
+    unfold has_instruction_type_checker in H; repeat my_auto5; by constructor.
+  - (* num, using destruct inst, withut have_instruction_type *)
+    unfold has_instruction_type_checker in H; repeat my_auto5; by constructor.
+  - (* numconst, using destruct inst, without have_instruction_type *)
+    unfold has_instruction_type_checker in H; repeat my_auto5.
+    apply has_num_type_type_correct in HMatch4. destruct HMatch4 as [ν HMatch4]; subst.
+    by constructor.
+  - admit.
+  - admit.
+  - Opaque have_instruction_type_checker.
+    unfold has_instruction_type_checker in H; repeat my_auto5.
+Admitted.
+
+Definition has_function_type_checker
+    (M:module_ctx) (mf:module_function) (ft:function_type) : type_checker_res :=
+  INR "incomplete".
+Lemma has_function_type_checker_correct :
+  ∀ M mf ft, has_function_type_checker M mf ft = ok_term ->
+             has_function_type M mf ft.
+Proof. Admitted.
+
+Definition has_module_type_checker (m:module) (mt:module_type) : type_checker_res :=
+  INR "incomplete".
+Lemma has_module_type_checker_correct :
+  ∀ m mt, has_module_type_checker m mt = ok_term -> has_module_type m mt.
+Proof. Admitted.
